CCsub_Soundness.v
@@ -1,5 +1,6 @@
 Require Import Coq.Program.Equality.
 Require Import TaktikZ.
+Require Import Lia.
 
 Require Import CCsub_Subcapt.
 Require Import CCsub_Subtyping.
@@ -8,118 +9,28 @@ Require Import CCsub_Substitution.
 
 Set Nested Proofs Allowed.
 
-(* States *)
-
-Inductive store_frame : Type :=
-  | store v : value v -> store_frame.
-
-Definition store_ctx : Type := list (atom * store_frame).
-Definition stores (S : store_ctx) (x : atom) (v : exp) (v_value : value v) : Prop :=
-    binds x (store v v_value) S.
-
-Inductive scope (e : exp) : Type :=
-  | mk_scope L : (forall x, x `notin` L -> expr (open_ve e x (`cset_fvar` x))) -> scope e.
-
-Inductive eval_frame : Type :=
-  | cont e : scope e -> eval_frame.
-
-Definition eval_ctx : Type := (list eval_frame).
-
-Inductive state : Type :=
-  | mk_state : store_ctx -> eval_ctx -> exp -> state.
-
-Notation "⟨ S | E | e ⟩" := (mk_state S E e) (at level 1).
-
-Inductive state_final : state -> Prop :=
-  | final_state : forall S a,
-      answer a ->
-      state_final ⟨ S | nil | a ⟩.
-
-Inductive store_typing : store_ctx -> env -> Prop :=
-  | typing_store_nil : store_typing nil nil
-  | typing_store_cons : forall x T v v_value S E,
-      store_typing S E ->
-      typing E v T ->
-      x `notin` dom E ->
-      store_typing ([(x, store v v_value)] ++ S) ([(x, bind_typ T)] ++ E).
-
-Inductive eval_typing (E : env) : eval_ctx -> typ -> typ -> Prop :=
-  | typing_eval_nil : forall T U,
-      wf_env E ->
-      sub E T U ->
-      eval_typing E nil T U
-  | typing_eval_cons : forall L k (k_scope : scope k) K T U V,
-      (forall x, x `notin` L ->
-        typing ([(x, bind_typ T)] ++ E) (open_ve k x (`cset_fvar` x)) U) ->
-      eval_typing E K U V ->
-      eval_typing E (cont k k_scope :: K) T V.
-
-Inductive state_typing : state -> typ -> Prop :=
-  | typing_state : forall S K e E T U,
-      store_typing S E ->
-      eval_typing E K T U ->
-      typing E e T ->
-      state_typing ⟨ S | K | e ⟩ U.
-
-(** TODO check where this is used and maybe use "wellformed" tactic **)
-Lemma wf_typ_extract_typ_arrow : forall C E T1 T2,
-  wf_typ_in E (typ_capt C (typ_arrow T1 T2)) ->
-  exists L, forall x, x `notin` L ->
-    wf_typ ([(x, bind_typ T1)] ++ E) (dom E `union` singleton x) (dom E) (open_ct T2 (`cset_fvar` x)).
-Proof with eauto.
-  intros * HWf.
-  inversion HWf; subst.
-  inversion H5; subst...
-Qed.
-
-(** TODO check where this is used and maybe use "wellformed" tactic **)
-Lemma typing_extract_typ_arrow : forall E e C T1 T2,
-  typing E e (typ_capt C (typ_arrow T1 T2)) ->
-  exists L, forall x, x `notin` L ->
-    wf_typ ([(x, bind_typ T1)] ++ E) (dom E `union` singleton x) (dom E) (open_ct T2 (`cset_fvar` x)).
-Proof with eauto.
-  intros * Htyp.
-  apply (wf_typ_extract_typ_arrow C)...
-Qed.
-
-(* ********************************************************************** *)
-(** ** Canonical forms (14) *)
-
-Lemma canonical_form_abs : forall e U1 U2 C,
-  value e ->
-  typing empty e (typ_capt C (typ_arrow U1 U2)) ->
-  exists V, exists e1, e = exp_abs V e1.
-Proof.
-  intros e U1 U2 C Val Typ.
-  remember empty.
-  remember (typ_arrow U1 U2).
-  revert U1 U2 Heqp Heql.
-  dependent induction Typ; intros U1 U2 EQT EQE; subst;
-    try solve [ inversion Val | inversion EQT | eauto ].
-  Case "typing_sub".
-  inversion H; subst; eauto.
-  + binds_cases H0.
-  + inversion H5; subst.
-    eapply IHTyp; eauto.
-Qed.
-
-Lemma canonical_form_tabs : forall e U1 U2 C,
-  value e ->
-  typing empty e (typ_capt C (typ_all U1 U2)) ->
-  exists V, exists e1, e = exp_tabs V e1.
-Proof.
-  intros e U1 U2 C Val Typ.
-  remember empty.
-  remember (typ_all U1 U2).
-  revert U1 U2 Heqp Heql.
-  dependent induction Typ; intros U1 U2 EQT EQE; subst;
-    try solve [ inversion Val | inversion EQT | eauto ].
-  Case "typing_sub".
-  inversion H; subst; eauto.
-  + binds_cases H0.
-  + inversion H5; subst.
-    eapply IHTyp; eauto.
-Qed.
+Tactic Notation "destructs" constr(E) :=
+  destruct ltac:(applys E).
+Tactic Notation "destructs" constr(E) "as" simple_intropattern(P) :=
+  destruct ltac:(applys E) as P.
+Tactic Notation "destructs" constr(E0) constr(A1) :=
+  destructs (>> E0 A1).
+Tactic Notation "destructs" constr(E0) constr(A1) "as" simple_intropattern(P) :=
+  destructs (>> E0 A1) as P.
+Tactic Notation "destructs" constr(E0) constr(A1) constr(A2) :=
+  destructs (>> E0 A1 A2).
+Tactic Notation "destructs" constr(E0) constr(A1) constr(A2) "as" simple_intropattern(P) :=
+  destructs (>> E0 A1 A2) as P.
+Tactic Notation "destructs" constr(E0) constr(A1) constr(A2) constr(A3) :=
+  destructs (>> E0 A1 A2 A3).
+Tactic Notation "destructs" constr(E0) constr(A1) constr(A2) constr(A3) "as" simple_intropattern(P) :=
+  destructs (>> E0 A1 A2 A3) as P.
+Tactic Notation "destructs" constr(E0) constr(A1) constr(A2) constr(A3) constr(A4) "as" simple_intropattern(P) :=
+  destructs (>> E0 A1 A2 A3 A4) as P.
+Tactic Notation "destructs" constr(E0) constr(A1) constr(A2) constr(A3) constr(A4) constr(A5) "as" simple_intropattern(P) :=
+  destructs (>> E0 A1 A2 A3 A4 A5) as P.
+Tactic Notation "destructs" constr(E0) constr(A1) constr(A2) constr(A3) constr(A4) constr(A5) constr(A6) "as" simple_intropattern(P) :=
+  destructs (>> E0 A1 A2 A3 A4 A5 A6) as P.
 
 (* ********************************************************************** *)
 (** * #<a name="preservation"></a># Preservation *)
@@ -138,94 +49,38 @@ Proof with eauto.
   - exists C. exists P...
 Qed.
 
-(*
-Lemma typing_state_free_tvar : forall S E,
+Lemma no_type_bindings_cons : forall E x T,
+  no_type_bindings E ->
+  no_type_bindings ([(x, bind_typ T)] ++ E).
+Proof with eauto*.
+  intros * NTB.
+  intros y U.
+  intros Binds.
+  binds_cases Binds.
+  apply (NTB y U), H.
+Qed.
+
+Lemma no_type_bindings_strengthening : forall F E,
+  ok (F ++ E) ->
+  no_type_bindings (F ++ E) ->
+  no_type_bindings E.
+Proof with eauto*.
+  intros * Ok NTB.
+  intros X U Binds.
+  eapply binds_weaken_at_head in Binds...
+  apply (NTB X U Binds).
+Qed.
+
+Lemma store_typing_no_type_bindings : forall S E,
   store_typing S E ->
   no_type_bindings E.
-Proof with eauto.
-  intros. unfold no_type_bindings; intros.
-  induction H...
-  * intro. binds_cases H...
-  * intro.s 
-Qed.
-*)
-
-Fixpoint env_fv_ct (F : env) {struct F} : atoms :=
-  match F with
-  | nil => {}A
-  | (_, bind_typ T) :: F' => (fv_ct T) `u`A (env_fv_ct F')
-  | (_, bind_sub T) :: F' => (fv_ct T) `u`A (env_fv_ct F')
-  end.
-
-Lemma stores_unique : forall S x v1 v1_value v2 v2_value,
-  stores S x v1 v1_value ->
-  stores S x v2 v2_value ->
-  v1 = v2.
 Proof with eauto*.
-  intros * stores1 stores2.
-  unfold stores, binds in *.
-  rewrite stores1 in stores2.
-  inversion stores2...
-Qed.
-
-Lemma wf_cset_notin_fvars : forall x E A C,
-  wf_cset E A C ->
-  x `~in`A dom E ->
-  x `~in`A (`cset_fvars` C).
-Proof with eauto*.
-  intros * WfC NotIn.
-  induction WfC.
-  enough (fvars `c`A dom E) by fsetdec.
-  intros y yIn.
-  destruct (H y ltac:(fsetdec)) as [T [B|B]]; eapply binds_In...
-Qed.
-
-Lemma wf_typ_notin_fv_ct : forall x E Ap Am T,
-  wf_typ E Ap Am T ->
-  x `~in`A dom E ->
-  x `~in`A fv_ct T
-with wf_pretyp_notin_fv_cpt : forall x E Ap Am P,
-  wf_pretyp E Ap Am P ->
-  x `~in`A dom E ->
-  x `~in`A fv_cpt P.
-Proof with eauto*.
-{ intros * WfT NotIn.
-  induction WfT; simpl.
-  - fsetdec.
-  - assert (x `~in`A (`cset_fvars` C)) by (applys wf_cset_notin_fvars; eauto*).
-    assert (x `~in`A fv_cpt P) by (applys wf_pretyp_notin_fv_cpt; eauto*).
-    fsetdec.
-}
-{ intros * WfP NotIn.
-  induction WfP; simpl.
-  - fsetdec.
-  - assert (x `~in`A fv_ct T1) by (applys wf_typ_notin_fv_ct; eauto*).
-    pick fresh y and specialize H0.
-    assert (x `~in`A fv_ct T2).
-    { eapply notin_fv_ct_open_ct.
-      eapply wf_typ_notin_fv_ct.
-      apply H0.
-      simpl.
-      assert (x <> y) by (clear - Fr; fsetdec).
-      clear Fr.
-      fsetdec.
-    }
-    clear - H1 H2.
-    fsetdec.
-  - assert (x `~in`A fv_ct T1) by (applys wf_typ_notin_fv_ct; eauto*).
-    pick fresh y and specialize H0.
-    assert (x `~in`A fv_ct T2).
-    { eapply notin_fv_ct_open_tt.
-      eapply wf_typ_notin_fv_ct.
-      apply H0.
-      simpl.
-      assert (x <> y) by (clear - Fr; fsetdec).
-      clear Fr.
-      fsetdec.
-    }
-    clear - H1 H2.
-    fsetdec.
-}
+  intros * StoreTyp.
+  induction StoreTyp.
+  - easy.
+  - intros X U Binds.
+    binds_cases Binds.
+    applys IHStoreTyp H1.
 Qed.
 
 Lemma wf_env_bound_implies_wf_typ : forall E x T,
@@ -276,203 +131,6 @@ Proof with eauto*.
         apply wf_typ_in_weakening...
         apply ok_cons... 
 Qed.
-
-Lemma wf_typ_in_notin_fv_ct : forall x E T,
-  wf_typ_in E T ->
-  x `~in`A dom E ->
-  x `~in`A fv_ct T
-with wf_pretyp_in_notin_fv_cpt : forall x E P,
-  wf_pretyp_in E P ->
-  x `~in`A dom E ->
-  x `~in`A fv_cpt P.
-Proof with eauto*.
-{ intros * WfT NotIn.
-  eapply wf_typ_notin_fv_ct with (E := E) (Ap := dom E) (Am := dom E)...
-}
-{ intros * WfP NotIn.
-  eapply wf_pretyp_notin_fv_cpt with (E := E) (Ap := dom E) (Am := dom E)...
-}
-Qed.
-
-(*
-Lemma typing_of_var_comes_from_binds : forall E (x : atom) T,
-  typing E x T ->
-  exists S, binds x (bind_typ S) E /\ sub E S T.
-Proof with eauto using sub_reflexivity, sub_transitivity.
-  intros * Typ.
-  destruct (typing_regular _ _ _ Typ) as [_ [_ WfT]].
-  dependent induction Typ.
-  - Case "typing_var_tvar".
-    exists X; split...
-  - Case "typing_var".
-    exists (typ_capt C P); split...
-    assert (WfC : wf_cset_in E C).
-    { enough (WfCP : wf_typ_in E (typ_capt C P)) by (inversion WfCP; eauto* ).
-      applys wf_env_binds_typ_implies_wf_typ H H0.
-    }
-    apply sub_capt.
-    + inversion WfC; subst.
-      admit.
-    + eapply sub_pre_reflexivity...
-      inversion WfT...
-      all: clear; fsetdec.
-  - Case "typing_sub".
-    destruct (IHTyp x) as [R [x_binds_R sub_R]]...
-    exists R; split.
-    + apply x_binds_R.
-    + apply sub_transitivity with (Q := S)...
-Admitted.
-*)
-
-(* TODO: move to infrastructure *)
-Lemma notin_open_ve_rec_fv_ve : forall k y z C e,
-  y `notin` (fv_ve e `union` singleton z) ->
-  y `notin` fv_ve (open_ve_rec k z C e).
-Proof with eauto*.
-  intros * y_notin_e_z.
-  generalize dependent k.
-  induction e; intros k; simpl in *;
-  repeat match goal with
-  | v : var |- _ =>
-      destruct v; simpl in *; eauto*;
-      destruct (k === n); eauto*
-  | |- y `notin` (_ `union` _) => apply notin_union
-  | IH : y `notin` _ -> forall k, _ |- _ => apply IH; eauto*
-  end.
-Qed.
-
-Lemma notin_open_te_rec_fv_ve : forall k y z e,
-  y `notin` (fv_ve e `union` singleton z) ->
-  y `notin` fv_ve (open_te_rec k z e).
-Proof with eauto*.
-  intros * y_notin_e_z.
-  generalize dependent k.
-  induction e; intros k; simpl in *;
-  repeat match goal with
-  | v : var |- _ =>
-      destruct v; simpl in *; eauto*;
-      destruct (k === n); eauto*
-  | |- y `notin` (_ `union` _) => apply notin_union
-  | IH : y `notin` _ -> forall k, _ |- _ => apply IH; eauto*
-  end.
-Qed.
-
-Lemma sub_implies_subcapt_cv : forall E S T,
-  sub E S T ->
-  subcapt E (cv S) (cv T).
-Proof with eauto*.
-  intros * Sub.
-  induction Sub; simpl.
-  - apply subcapt_reflexivity with (A := dom E)...
-    constructor.
-    + intros x xIn.
-      assert (x = X) by fsetdec; subst; clear xIn.
-      inversion H0; subst.
-      exists U.
-      apply bound_sub, H2.
-    + inversion H0; subst.
-      fsetdec.
-  - eapply subcapt_tvar with (T := U)...
-  - assumption.
-Qed.
-
-Lemma binds_wf : forall E x T,
-  wf_env E ->
-  binds x (bind_typ T) E ->
-  wf_typ E (dom E `\`A x) (dom E `\`A x) T.
-Proof with eauto*.
-  intros * WfE Binds.
-  induction WfE; simpl.
-  - inversion Binds.
-  - rewrite_env (empty ++ [(X, bind_sub T0)] ++ E).
-    assert (x <> X).
-    { inversion Binds.
-      destruct (x == X)... }
-    replace (({X}A `u`A dom E) `\`A x) with ((dom E `\`A x) `u`A {X}A) by fsetdec.
-    apply wf_typ_weakening with (Ap := dom E `\`A x) (Am := dom E `\`A x).
-    + apply IHWfE.
-      inversion Binds.
-      destruct (x == X)...
-    + apply ok_cons...
-    + fsetdec.
-    + fsetdec.
-  - inversion Binds.
-    destruct (x == x0); subst.
-    + inversion H2; subst.
-      replace (({x0}A `u`A dom E) `\`A x0) with (dom E) by fsetdec.
-      rewrite_env (empty ++ [(x0, bind_typ T)] ++ E).
-      apply wf_typ_weakening with (Ap := dom E) (Am := dom E)...
-      apply ok_cons...
-    + rewrite_env (empty ++ [(x0, bind_typ T0)] ++ E).
-      replace (({x0}A `u`A dom E) `\`A x) with ((dom E `\`A x) `u`A {x0}A) by fsetdec.
-      apply wf_typ_weakening with (Ap := dom E `\`A x) (Am := dom E `\`A x).
-      * apply IHWfE...
-      * apply ok_cons...
-      * fsetdec.
-      * fsetdec.
-Qed.
-
-Lemma wf_cset_notin_fvars_atoms : forall E Ap x C,
-  wf_cset E Ap C ->
-  x `~in`A Ap ->
-  x `~in`A (`cset_fvars` C).
-Proof with eauto*.
-  intros * WfC NotIn.
-  inversion WfC; subst...
-Qed.
-
-Lemma wf_typ_notin_cv : forall E Ap Am x T,
-  wf_typ E Ap Am T ->
-  x `~in`A Ap ->
-  x `~in`A (`cset_fvars` (cv T)).
-Proof with eauto*.
-  intros * WfT NotIn.
-  induction WfT; simpl...
-  apply wf_cset_notin_fvars_atoms with (E := E) (Ap := Ap)...
-Qed.
-
-(*
-Lemma subcapt_notin_fvars : forall E C D x,
-  wf_env E ->
-  subcapt E C D ->
-  x `~in`A (`cset_fvars` D) ->
-  `* in` D \/ x `~in`A (`cset_fvars` C).
-Proof with eauto*.
-  intros * WfE Subcapt NotIn.
-  induction Subcapt; subst; simpl in *.
-  - left...
-  - right...
-  - left...
-  - destruct (IHSubcapt WfE NotIn).
-    + left...
-    + right.
-      enough (x <> x0) by fsetdec.
-      intros eq; subst.
-      assert (WfT : wf_typ E (dom E `\`A x0) (dom E `\`A x0) T) by (applys binds_wf WfE H; eauto* ).
-      assert ()
-      
-
-Lemma sub_notin_fv_ct : forall E S T x,
-  sub E S T ->
-  x `~in`A fv_ct T ->
-  x `~in`A fv_ct S
-with sub_pre_notin_fv_ctp : forall E P Q x,
-  sub_pre E P Q ->
-  x `~in`A fv_cpt P ->
-  x `~in`A fv_cpt Q.
-Proof with eauto*.
-{ intros * Sub NotIn.
-  induction Sub; simpl in *.
-  - apply notin_empty.
-  - apply notin_empty.
-  - apply notin_union.
-    +  
-}
-{ intros * Sub NotIn.
-  Guarded.
-
-}
-*)
 
 Lemma typing_strengthening : forall F E x U e T,
   x `~in`A (fv_cctx F `u`A fv_ct T `u`A fv_ve e) ->
@@ -731,43 +389,6 @@ Proof with eauto*.
       * fsetdec.
 Admitted.
 
-Lemma typing_var_inversion : forall E (x : atom) T,
-  typing E x T ->
-     (exists C P, binds x (bind_typ (typ_capt C P)) E /\ sub E (typ_capt (`cset_fvar` x) P) T)
-  \/ (exists X : atom, binds x (bind_typ X) E /\ sub E X T).
-Proof with eauto*.
-  intros * Typ.
-  dependent induction Typ.
-  - Case "typing_var_tvar".
-    right.
-    exists X.
-    split...
-    apply sub_refl_tvar...
-    apply wf_env_bound_implies_wf_typ with (x := x)...
-  - Case "typing_capt".
-    left.
-    exists C, P.
-    split...
-    apply sub_reflexivity with (Ap := dom E) (Am := dom E)...
-    apply wf_typ_capt.
-    + apply wf_concrete_cset.
-      * intros y yIn; assert (y = x) by (clear - yIn; fsetdec); subst...
-      * enough (x `in`A dom E) by fsetdec.
-        eapply binds_In... 
-    + enough (WfCP : wf_typ_in E (typ_capt C P)) by (inversion WfCP; eauto*).
-      apply wf_env_bound_implies_wf_typ with (x := x)...
-  - Case "typing_sub".
-    destruct (IHTyp x eq_refl) as [[C [P [xBinds Sub]]] | [X [xBinds Sub]]].
-    + left.
-      exists C, P.
-      split...
-      apply sub_transitivity with (Q := S)...
-    + right.
-      exists X.
-      split...
-      apply sub_transitivity with (Q := S)...
-Qed.
-
 Lemma sub_capt_inversion : forall E C P T,
   sub E (typ_capt C P) T ->
   exists D Q, T = typ_capt D Q
@@ -776,110 +397,6 @@ Lemma sub_capt_inversion : forall E C P T,
 Proof with eauto*.
   intros * Sub; inversion Sub...
 Qed.
-
-Inductive binds_sub_trans : atom -> cap -> pretyp -> env -> Prop :=
-  | binds_sub_trans_concrete : forall E X C P,
-      binds X (bind_sub (typ_capt C P)) E ->
-      binds_sub_trans X C P E
-  | binds_sub_trans_indirect : forall E (X Y : atom) C P,
-      binds X (bind_sub Y) E ->
-      binds_sub_trans Y C P E ->
-      binds_sub_trans X C P E.
-
-Inductive binds_typ_trans : atom -> cap -> pretyp -> env -> Prop :=
-  | binds_typ_trans_concrete : forall E x C P,
-      binds x (bind_typ (typ_capt C P)) E ->
-      binds_typ_trans x C P E
-  | binds_typ_trans_indirect : forall E (x X : atom) C P,
-      binds x (bind_typ X) E ->
-      binds_sub_trans X C P E ->
-      binds_typ_trans x C P E.
-
-Hint Constructors binds_sub_trans binds_typ_trans : core.
-
-Lemma binds_sub_trans_weakening : forall G F E X C P,
-  ok (G ++ F ++ E) ->
-  binds_sub_trans X C P (G ++ E) ->
-  binds_sub_trans X C P (G ++ F ++ E).
-Proof with eauto*.
-  intros * OkGFE Binds.
-  dependent induction Binds...
-Qed.
-
-(*
-Lemma sub_var_capt_inversion : forall E (X : atom) C P,
-  sub E X (typ_capt C P) ->
-  exists D Q, binds_sub_trans X D Q E
-           /\ subcapt E D C
-           /\ sub_pre E Q P.
-Proof with eauto*.
-  intros * Sub.
-  assert (WfEnv : wf_env E) by applys sub_regular Sub.
-  generalize dependent X.
-  induction WfEnv; intros X0 Sub; inversion Sub; subst.
-  - inversion H0.
-  - destruct (X0 == X); subst.
-    + inversion H2; subst.
-      destruct (X == X); try (contradict n; reflexivity).
-      inversion H3; subst.
-      clear e H3 H2.
-      admit.
-    + 
-*)
-
-(*
-Lemma typing_var_capt_inversion : forall E (x : atom) C P,
-  typing E x (typ_capt C P) ->
-  exists D Q, binds x (bind_typ (typ_capt D Q)) E
-           /\ subcapt E (`cset_fvar` x) C
-           /\ sub_pre E P Q.
-Proof with eauto*.
-  intros * Typ.
-  dependent induction Typ.
-  - exists C0, P.
-    repeat split...
-    + apply subcapt_reflexivity with (A := dom E)...
-      econstructor.
-      * intros z zIn; assert (z = x) by (clear - zIn; fsetdec); subst...
-      * enough (x `in`A dom E) by fsetdec.
-        apply binds_In with (a := bind_typ (typ_capt C0 P))...
-    + apply sub_pre_reflexivity with (Ap := dom E) (Am := dom E)...
-      enough (WfC0P : wf_typ_in E (typ_capt C0 P)) by (inversion WfC0P; eauto* ).
-      apply wf_env_bound_implies_wf_typ with (x := x)...
-  - 
-  eremember (typ_capt C P) as T.
-  assert (Sub : sub E T (typ_capt C P)).
-  { subst; apply sub_reflexivity with (Ap := dom E) (Am := dom E)...
-    applys typing_regular Typ.
-  }
-  clear HeqT.
-  dependent induction Typ.
-  - Case "typing_var_tvar".
-    exists C, P.
-    repeat split...
-    + apply binds_typ_trans_indirect with (X := X)...
-      apply binds_sub_trans_concrete.
-  - exists C0, P.
-    repeat split...
-    + apply subcapt_reflexivity with (A := dom E)...
-      constructor.
-      * intros z zIn; assert (z = x) by (clear - zIn; fsetdec); subst; clear zIn...
-      * enough (x `in`A dom E) by fsetdec; apply binds_In with (a := bind_typ (typ_capt C0 P))...
-    + apply sub_pre_reflexivity with (Ap := dom E) (Am := dom E)...
-      enough (WfC0P : wf_typ_in E (typ_capt C0 P)) by (inversion WfC0P; eauto* ).
-      apply wf_env_bound_implies_wf_typ with (x := x)...
-  - 
-*)
-
-(*
-Lemma typing_var_induction : forall E (x : atom) T,
-  typing E x T ->
-  (exists P, sub E (typ_capt (`cset_fvar` x) P) T).
-Proof with eauto*.
-  intros * Typ.
-  dependent induction Typ.
-  -  
-*)
 
 Ltac impossible_typing Typ :=
   clear - Typ;
@@ -897,245 +414,6 @@ Ltac impossible_typing Typ :=
             eapply IH; [ eauto | eapply sub_transitivity with (Q := T); eauto* ]; trivial
         end ]
   end.
-
-Lemma subcapt_binds : forall x C P E D,
-  wf_env E ->
-  wf_cset_in E C ->
-  wf_pretyp_in E P ->
-  x `~in`A (`cset_fvars` D) ->
-  subcapt ([(x, bind_typ (typ_capt C P))] ++ E) (`cset_fvar` x) D ->
-  subcapt E C D.
-Proof with eauto*.
-  intros * WfE WfC WfP NotIn Sub.
-  dependent induction Sub.
-  - Case "subcapt_universal".
-    apply subcapt_universal...
-    apply wf_concrete_cset.
-    + intros z zIn.
-      inversion H; subst.
-      destruct (H5 z ltac:(fsetdec)) as [T [B|B]]; binds_cases B...
-    + inversion H; subst.
-      rewrite dom_concat in H6; simpl in H6.
-      fsetdec.
-  - Case "subcapt_in".
-    inversion WfC; subst.
-    admit.
-    (* eapply subcapt_set.
-    assert (x0 = x1) by (apply singleton_set_eq, x); subst; clear x H1.
-    apply subcapt_transitivity with (C2 := `cset_fvar` x1)... *)
-  - Case "subcapt_in_univ".
-    admit.
-  - Case "subcapt_var".
-    admit.
-  - Case "subcapt_set".
-    admit.
-Admitted.
-
-Lemma idk : forall x C P E T, 
-  sub ([(x, bind_typ (typ_capt C P))] ++ E) (typ_capt (`cset_fvar` x) P) T ->
-  sub E (typ_capt C P) T.
-Proof with eauto*.
-  intros * Sub.
-  assert (WfEnv : wf_env ([(x, bind_typ (typ_capt C P))] ++ E)) by applys sub_regular Sub.
-  inversion WfEnv; subst; clear WfEnv.
-  inversion H3; subst; clear H3.
-  rename H2 into WfE.
-  rename H4 into NotIn.
-  rename H7 into WfC.
-  rename H8 into WfP.
-  dependent induction Sub.
-  apply sub_capt.
-  - admit.
-  - admit.
-Admitted.
-
-Lemma sub_tvar_inversion : forall E T (X : atom),
-  sub E T X ->
-  exists Y : atom, T = X \/ binds Y (bind_sub X) E.
-Proof with eauto*.
-  intros * Sub.
-  dependent induction Sub...
-  destruct (IHSub X ltac:(reflexivity)) as [Y [Eq | Binds]]; subst.
-  - exists X0. right. apply H.
-  - exists Y. right. apply Binds.
-  Unshelve.
-  apply X.
-Qed.
-
-Lemma sub_pre_arrow_inversion : forall E T1 T2 P,
-  sub_pre E (typ_arrow T1 T2) P ->
-  P = typ_top
-  \/ (exists S1 S2 L, P = typ_arrow S1 S2
-     /\ sub E S1 T1
-     /\ (forall x, x `~in`A L ->
-           sub ([(x, bind_typ S1)] ++ E)
-               (open_ct T2 (`cset_fvar` x))
-               (open_ct S2 (`cset_fvar` x)))).
-Proof with eauto*.
-  intros * Sub.
-  dependent induction Sub...
-  right.
-  exists T0, T3, L.
-  repeat split...
-Qed.
-
-Lemma sub_capt_arrow_inversion : forall E C T1 T2 T,
-  sub E (typ_capt C (typ_arrow T1 T2)) T ->
-  exists D, T = typ_capt D typ_top
-  \/ (exists S1 S2 L, T = typ_capt D (typ_arrow S1 S2)
-     /\ subcapt E C D
-     /\ sub E S1 T1
-     /\ (forall x, x `~in`A L ->
-          sub ([(x, bind_typ S1)] ++ E)
-              (open_ct T2 (`cset_fvar` x))
-              (open_ct S2 (`cset_fvar` x)))).
-Proof with eauto*.
-  intros * Sub.
-  dependent induction Sub.
-  destruct (sub_pre_arrow_inversion _ _ _ _ H0) as [Eq | [S1 [S2 [L [Eq [S1SubT1 T2SubS2]]]]]]; subst.
-  - exists C2...
-  - exists C2.
-    right.
-    exists S1, S2.
-    repeat split...
-Qed.
-
-Lemma typing_abs_implies_sub_arrow : forall E U e T,
-  typing E (exp_abs U e) T ->
-  exists T1 T2, typing E (exp_abs U e) (typ_capt (free_for_cv e) (typ_arrow T1 T2))
-             /\ sub E (typ_capt (free_for_cv e) (typ_arrow T1 T2)) T.
-Proof with eauto*.
-  intros * Typ.
-  assert (WfEnv : wf_env E) by applys typing_regular Typ.
-  assert (WfCV : wf_cset_in E (free_for_cv (exp_abs U e))).
-  { eapply typing_cv... }
-  simpl in WfCV.
-  dependent induction Typ.
-  - exists U, T1.
-    split...
-    apply sub_reflexivity with (Ap := dom E) (Am := dom E)...
-  - destruct (IHTyp U e ltac:(reflexivity) WfEnv WfCV) as [T1 [T2 Sub]].
-    exists T1, T2.
-    split...
-    apply sub_transitivity with (Q := S)...
-Qed.
-
-(*
-Lemma typing_abs_all_impossible : forall E U e C T1 T2,
-  ~ typing E (exp_abs U e) (typ_capt C (typ_all T1 T2)).
-Proof with eauto*.
-  intros * Typ.
-  dependent induction Typ.
-
-Lemma typing_val_inversion_aux : forall E v T,
-  value v ->
-  typing E v T ->
-  exists C P, T = typ_capt C P
-  /\ (P = typ_top
-   \/ (exists T1 T2, P = typ_arrow T1 T2)
-   \/ (exists T1 T2, P = typ_all T1 T2)).
-Proof with eauto*.
-  intros * Val Typ.
-  assert (WfEnv : wf_env E) by applys typing_regular Typ.
-  assert (WfCV : wf_cset_in E (free_for_cv v)) by applys typing_cv Typ.
-  inversion Val; subst.
-  - dependent induction Typ...
-    + exists (free_for_cv e1), (typ_arrow T0 T1).
-      repeat split...
-    + destruct (IHTyp T0 e1 ltac:(reflexivity) Val WfEnv WfCV H0) as [C [P [EqS [EqP | [[T2 [T3 EqP]] | [T2 [T3 EqP]]]]]]]; subst.
-      * inversion H; subst.
-        inversion H6; subst.
-        exists C2, typ_top...
-      * inversion H; subst.
-        inversion H6; subst.
-        -- exists C2, typ_top...
-        -- exists C2, (typ_arrow T1 T4)...
-      * inversion Typ; subst.
-        inversion H6; subst.
-        -- exists  
-  - dependent induction Typ...
-    exists (free_for_cv e1), (typ_all T0 T1)...
-
-Lemma typing_val_inversion : forall E v T,
-  value v ->
-  typing E v T ->
-  exists C P, typing E v (typ_capt C P)
-  /\ sub E T (typ_capt C P)
-  /\ ((exists T1 T2, P = typ_arrow T1 T2)
-   \/ (exists T1 T2, P = typ_all T1 T2)).
-Proof with eauto*.
-  intros * Val Typ.
-  assert (WfEnv : wf_env E) by applys typing_regular Typ.
-  assert (WfCV : wf_cset_in E (free_for_cv v)) by applys typing_cv Typ.
-  inversion Val; subst.
-  - dependent induction Typ...
-    + exists (free_for_cv e1), (typ_arrow T0 T1).
-      repeat split...
-      apply sub_reflexivity with (Ap := dom E) (Am := dom E)...
-    + destruct (IHTyp T0 e1 ltac:(reflexivity) Val WfEnv WfCV H0) as [C [P [Typ' [Sub' [[T2 [T3 Eq]] | [T2 [T3 Eq]]]]]]]; subst.
-      * repeat eexists.
-  - dependent induction Typ...
-    exists (free_for_cv e1), (typ_all T0 T1)...
-Qed.
-*)
-
-Lemma typing_var_concrete_tvar_impossible : forall E x C P (X : atom),
-  binds x (bind_typ (typ_capt C P)) E ->
-  ~ typing E x X.
-Proof with eauto*.
-  intros * Binds Typ.
-  dependent induction Typ...
-  dependent induction H...
-Qed.
-
-Lemma typing_lift_cpt_to_capt : forall E e C P,
-  typing E e (typ_capt C P) ->
-  exists Q, typing E e (typ_capt (C `u` cset_set (fv_cpt P) {}N false) Q)
-         /\ sub_pre E Q P
-         /\ (fv_cpt Q) `disjoint` (fv_ve e).
-Proof with eauto*.
-  (* REVIEW: is this true? *)
-Abort.
-
-Lemma store_typing_no_type_bindings : forall S E,
-  store_typing S E ->
-  no_type_bindings E.
-Proof with eauto*.
-  intros * StoreTyp.
-  induction StoreTyp.
-  - easy.
-  - intros X U Binds.
-    binds_cases Binds.
-    applys IHStoreTyp H1.
-Qed.
-
-Lemma binds_typ_implies_binds_capt : forall E x T,
-  no_type_bindings E ->
-  wf_env E ->
-  binds x (bind_typ T) E ->
-  exists C P, T = typ_capt C P.
-Proof with eauto*.
-  intros * NTB WfEnv Binds.
-  destruct T.
-  - exists c, p...
-  - enough (Wfn : wf_typ_in E n) by inversion Wfn.
-    apply wf_env_bound_implies_wf_typ with (x := x)...
-  - assert (Wfa : wf_typ_in E a) by (apply wf_env_bound_implies_wf_typ with (x := x); auto).
-    inversion Wfa; subst.
-    contradict H0.
-    apply (NTB a U).
-Qed.
-
-Lemma no_type_bindings_cons : forall E x T,
-  no_type_bindings E ->
-  no_type_bindings ([(x, bind_typ T)] ++ E).
-Proof with eauto*.
-  intros * NTB.
-  intros y U.
-  intros Binds.
-  binds_cases Binds.
-  apply (NTB y U), H.
-Qed.
 
 Lemma sub_left_capt_inversion : forall E T C P,
   no_type_bindings E ->
@@ -1164,7 +442,8 @@ Proof with eauto*.
     destruct (values_have_precise_captures _ _ _ v_value H) as [Q [TypQ QSubT]].
     assert (WfEnv : wf_env ([(x0, bind_typ T)] ++ E)) by applys typing_regular Typ.
     assert (NTB : no_type_bindings E) by applys store_typing_no_type_bindings StoreTyp.
-    destruct (binds_typ_implies_binds_capt ([(x0, bind_typ T)] ++ E) x0 T (no_type_bindings_cons E x0 T NTB) WfEnv ltac:(apply binds_head; auto)) as [D [R Eq]].
+    assert (WfT : wf_typ_in E T) by (inversion WfEnv; subst; auto).
+    destructs inversion_toplevel_type NTB WfT as [D [R Eq]].
     exists D, R.
     repeat split.
     + rewrite_env (empty ++ [(x0, bind_typ T)] ++ E).
@@ -1189,41 +468,6 @@ Proof with eauto*.
         fsetdec.
     + destruct (sub_capt_inversion _ _ _ _ QSubT) as [D' [R' [Eq' [CSubD QSubR]]]]; subst.
       symmetry in Eq'; inversion Eq'; subst; clear Eq'.
-      (*
-      assert (RSubP : sub_pre ([(x0, bind_typ (typ_capt D R))] ++ E) R P).
-      { clear - Typ.
-        dependent induction Typ.
-        - inversion H0; subst.
-          destruct (x0 == x0); try (contradict n; reflexivity).
-          inversion H2; subst.
-          clear e H2.
-          apply sub_pre_reflexivity with (Ap := dom ([(x0, bind_typ (typ_capt C0 P))] ++ E)) (Am := dom ([(x0, bind_typ (typ_capt C0 P))] ++ E))...
-          enough (WfC0P : wf_typ_in ([(x0, bind_typ (typ_capt C0 P))] ++ E) (typ_capt C0 P)) by (inversion WfC0P; auto).
-          apply wf_env_bound_implies_wf_typ with (x := x0)...
-        - inversion H; subst.
-          dependent induction H.
-          + contradict Typ; eapply typing_var_concrete_tvar_impossible...
-          + assert (WfEnv : wf_env ([(x0, bind_typ (typ_capt D R))] ++ E)) by applys typing_regular Typ.
-            inversion WfEnv; subst.
-            assert (RSubP1 : sub_pre ([(x0, bind_typ (typ_capt D R))] ++ E) R P1) by (eapply IHTyp with (x1 := x0) (C := C1); auto).
-            assert (x0 `~in`A fv_cpt P1).
-            { eapply wf_pretyp_notin_fv_cpt with (E := E) (Ap := dom E) (Am := dom E).
-              - rewrite_env (empty ++ E).
-                apply wf_pretyp_in_strengthen_typ with (x := x0) (U := typ_capt D R).
-                + csetsimpl.
-                  apply notin_union.
-                  * admit.
-                  * apply H7. 
-                + applys sub_pre_regular RSubP1.
-              - apply H7.
-            }
-            apply sub_pre_transitivity with (Q := P1).
-            * eapply pretype_from_wf_pretyp.
-              applys sub_pre_regular H5.
-            * eapply IHTyp with (x1 := x0) (C := C1)...
-            * apply wf_typ_notin_fv_ct with (x := x0) in H6; simpl in H6...
-      }
-      *)
       apply sub_pre_transitivity with (Q := R).
       * eapply pretype_from_wf_pretyp.
         applys sub_pre_regular QSubR.
@@ -1271,35 +515,35 @@ Proof with eauto*.
       * admit.
 Admitted.
 
-Lemma eval_typing_regular : forall E K T U,
-  eval_typing E K T U ->
-  wf_env E /\ wf_typ_in E T /\ wf_typ_in E U.
+Lemma eval_typing_sub : forall E K S1 S2 T1 T2,
+  no_type_bindings E ->
+  sub E S2 S1 ->
+  eval_typing E K S1 T1 ->
+  sub E T1 T2 ->
+  eval_typing E K S2 T2.
 Proof with eauto*.
-  intros * EvalTyp.
-  induction EvalTyp; repeat split...
-  pick fresh x and specialize H.
-  destruct (typing_regular _ _ _ H) as [wf_xTE _].
-  inversion wf_xTE; subst...
+  intros * NTB S2SubS1 EvalTyp T1SubT2.
+  revert S2 T2 S2SubS1 T1SubT2.
+  induction EvalTyp; intros S2 T2 S2SubT USubT2.
+  - Case "typing_eval_nil".
+    apply typing_eval_nil...
+    apply sub_transitivity with (Q := T)... 
+    apply sub_transitivity with (Q := U)...
+  - Case "typing_eval_cons".
+    eapply typing_eval_cons with (U := U) (L := L)...
+    + intros x NotIn.
+      rewrite_env (empty ++ [(x, bind_typ S2)] ++ E).
+      eapply typing_narrowing_typ_aux with (Q := T)...
+      destruct (sub_regular _ _ _ S2SubT) as [_ [WfS2 WfT]].
+      inversion WfS2; subst.
+      contradict H0; apply NTB.
+      inversion WfT; subst.
+      contradict H2; apply NTB.
+      constructor.
+    + apply IHEvalTyp...
+      apply sub_reflexivity with (Ap := dom E) (Am := dom E)...
+      applys eval_typing_regular EvalTyp.
 Qed.
-
-(*
-Lemma eval_typing_contravariant : forall E K S T U,
-  sub Γ S T ->
-  eval_typing E K T U ->
-  eval_typing E K S U.
-Proof with eauto*.
-  intros *.
-  intros subT eval_typ.
-  generalize dependent T'.
-  induction eval_typ; intros T' subT.
-  - apply typing_eval_nil...
-    apply sub_transitivity with (Q := T)...
-  - eapply typing_eval_cons with (L := L) (U := U)...
-    intros x x_fresh.
-    rewrite_env (empty ++ [(x, bind_typ T')] ++ Γ).
-    eapply typing_specializing...
-Qed.
-*)
 
 Lemma eval_typing_weakening : forall E F G E' T U,
   eval_typing (G ++ E) E' T U ->
@@ -1345,54 +589,6 @@ Proof with eauto*.
     + assumption.
 Qed.
 
-Lemma wf_capt_from_typing_var : forall E x C P,
-  wf_env E ->
-  binds x (bind_typ (typ_capt C P)) E ->
-  wf_cset_in E C /\ wf_pretyp_in E P.
-Proof with eauto*.
-  intros * WfEnv xBinds.
-  induction WfEnv.
-  - Case "wf_env_empty".
-    inversion xBinds.
-  - Case "wf_env_sub".
-    rewrite_env (empty ++ [(X, bind_sub T)] ++ E).
-    assert (binds x (bind_typ (typ_capt C P)) E).
-    { inversion xBinds.
-      destruct_if in H2...
-    }
-    destruct (IHWfEnv H1) as [WfC WfP].
-    split.
-    + apply wf_cset_in_weakening...
-      apply ok_cons...
-    + apply wf_pretyp_in_weakening...
-      apply ok_cons...
-  - Case "wf_env_typ".
-    destruct (x == x0); subst.
-    + SCase "x = x0".
-      inversion xBinds.
-      destruct (x0 == x0); try (contradict n; reflexivity).
-      inversion H2; subst.
-      rewrite_env (empty ++ [(x0, bind_typ (typ_capt C P))] ++ E).
-      split.
-      * apply wf_cset_in_weakening.
-        inversion H; subst...
-        apply ok_cons...
-      * apply wf_pretyp_in_weakening...
-        apply ok_cons...
-    + SCase "x <> x0".
-      rewrite_env (empty ++ [(x0, bind_typ T)] ++ E).
-      assert (binds x (bind_typ (typ_capt C P)) E).
-      { inversion xBinds.
-        destruct_if in H2...
-      }
-      destruct (IHWfEnv H1) as [WfC WfP].
-      split.
-      * apply wf_cset_in_weakening...
-        apply ok_cons...
-      * apply wf_pretyp_in_weakening...
-        apply ok_cons...
-Qed.
-
 Lemma typing_abs_typ_arrow_implies_sub_param : forall E U e C T1 T2,
   typing E (exp_abs U e) (typ_capt C (typ_arrow T1 T2)) ->
   sub E T1 U.
@@ -1415,433 +611,6 @@ Proof with eauto*.
     apply sub_transitivity with (Q := T)...
 Qed.
 
-Lemma binds_sub_arrow_implies_store_abs : forall S E C TFun T1 T2 f,
-  store_typing S E ->
-  binds f (bind_typ TFun) E ->
-  sub E TFun (typ_capt C (typ_arrow T1 T2)) ->
-  exists U e (abs_value : value (exp_abs U e)), stores S f (exp_abs U e) abs_value /\ sub E T1 U.
-Proof with eauto*.
-  intros * StoreTyp fBinds Sub.
-  eremember (typ_arrow T1 T2) as TFun' eqn:EQ.
-  induction StoreTyp; inversion fBinds; inversion EQ; subst.
-  destruct (f == x).
-  - inversion H2; subst...
-    unfold stores.
-    unfold binds.
-    simpl.
-    destruct (x == x); [ clear e | contradict n; reflexivity ].
-    inversion v_value; subst.
-    + inversion H; subst.
-      * exists T, e1, v_value.
-        inversion Sub; subst.
-        split...
-        inversion H13; subst...
-      * exists T, e1, v_value.
-        split...
-        rewrite_env (empty ++ [(x, bind_typ TFun)] ++ E).
-        apply sub_weakening.
-        -- assert (Typ : typing E (exp_abs T e1) (typ_capt C (typ_arrow T1 T2))).
-           { apply typing_sub with (S := TFun)...
-             rewrite_env (empty ++ [(x, bind_typ TFun)] ++ E) in Sub.
-             apply sub_strengthening in Sub.
-             - assumption.
-             - simpl.
-               repeat apply notin_union.
-               + clear; fsetdec.
-               + inversion Sub; subst.
-                 * clear; fsetdec.
-                 * destruct (sub_regular _ _ _ H5) as [_ [_ WfTyp]].
-                   eapply wf_typ_in_notin_fv_ct...
-               + eapply wf_cset_notin_fvars with (E := E) (A := dom E).
-                 * admit. 
-                 * apply H0.
-               + apply wf_typ_in_notin_fv_ct with (E := E).
-                 * admit.
-                 * apply H0.
-               + apply wf_typ_in_notin_fv_ct with (E := E).
-                 * admit.
-                 * apply H0.
-           }
-           applys typing_abs_typ_arrow_implies_sub_param Typ.
-        -- apply wf_env_typ...
-    + assert (tabs_has_type_T1_arr_T2 : typing E (exp_tabs T e1) (typ_capt C (typ_arrow T1 T2))).
-      { apply typing_sub with (S := TFun)...
-        rewrite_env (empty ++ [(x, bind_typ TFun)] ++ E) in Sub.
-        apply sub_strengthening in Sub.
-        - apply Sub.
-        - destruct (sub_regular _ _ _ Sub) as [WfEnv [WfTFun WfS]].
-          inversion WfEnv; inversion WfS. inversion H16; subst.
-          repeat apply notin_union.
-          + fsetdec.
-          + eapply wf_typ_in_notin_fv_ct...
-          + admit.
-          + admit.
-          + admit. 
-      }
-      admit.
-      (* exfalso; impossible_typing tabs_has_type_T1_arr_T2. *)
-  - assert (Sub' : sub E TFun (typ_capt C (typ_arrow T1 T2))).
-    { rewrite_env (empty ++ [(x, bind_typ T)] ++ E) in Sub.
-      apply sub_strengthening in Sub.
-      - apply Sub.
-      - repeat apply notin_union.
-        + fsetdec.
-        + admit.
-        + admit.
-        + admit.
-        + admit.     
-    }
-    destruct IHStoreTyp as [U [e [abs_value [xv_S_stores_f T1_sub_U]]]]...
-    exists U, e, abs_value.
-    split.
-    + rewrite_env ([(x, store v v_value)] ++ S).
-      apply binds_tail.
-      * trivial.
-      * simpl; fsetdec.
-    + rewrite_env (empty ++ [(x, bind_typ T)] ++ E).
-      apply sub_weakening...
-Admitted.
-
-(*
-Lemma subcapt_open_cset : forall E k C D c,
-  wf_cset_in E c ->
-  subcapt E C D ->
-  subcapt E (open_cset k C c) (open_cset k D c).
-Proof with eauto*.
-  intros * Wfc Subcapt.
-  unfold open_cset.
-  destruct (subcapt_regular _ _ _ Subcapt) as [WfC WfD].
-  inversion WfC; subst; rename H into HC, fvars into fvarsC.
-  inversion WfD; subst; rename H into HD, fvars into fvarsD.
-  destruct_set_mem k c.
-    induction Subcapt.
-    + csetsimpl.
-      Print open_cset.
-      replace (`cset_bvars` c `\`N k) with (`cset_bvars` c).
-      apply subcapt_universal.
-      * inversion H2; subst.
-  - eapply subcapt_reflexivity with (A := dom E)...
-
-Lemma sub_open_ct : forall E T C D,
-  wf_env E ->
-  wf_typ_in E T ->
-  subcapt E C D ->
-  sub E (open_ct T C) (open_ct T D)
-with sub_pre_open_cpt : forall E P C D,
-  wf_env E ->
-  wf_pretyp_in E P ->
-  subcapt E C D ->
-  sub_pre E (open_cpt P C) (open_cpt P D).
-Proof with eauto*.
-{ intros * WfEnv WfTyp Subcapt.
-  induction WfTyp; unfold open_ct; simpl.
-  - apply sub_refl_tvar...
-    apply wf_typ_var with (U := U)...
-    applys binds_In X...
-  - apply sub_capt.
-     
-}
-{ intros * Sub.
-}
-*)
-
-Lemma typing_inv_abs : forall E S1 e1 T,
-  typing E (exp_abs S1 e1) T ->
-  forall U1 U2 C, sub E T (typ_capt C (typ_arrow U1 U2)) ->
-    sub E U1 S1
-  /\ exists S2, exists L, forall x, x `notin` L ->
-    typing ([(x, bind_typ S1)] ++ E) (open_ve e1 x (`cset_fvar` x)) (open_ct S2 (`cset_fvar` x)) /\
-    wf_typ ([(x, bind_typ S1)] ++ E) (dom E `union` singleton x) (dom E) (open_ct U2 (`cset_fvar` x)) /\
-  sub ([(x, bind_typ U1)] ++ E) (open_ct S2 (`cset_fvar` x)) (open_ct U2 (`cset_fvar` x)).
-Proof with auto.
-  intros * Htyp.
-  dependent induction Htyp; intros U1 U2 C Hsub.
-  - Case "typing_abs".
-    inversion Hsub; subst.
-    inversion select (sub_pre _ _ _); subst.
-    split...
-    exists T1.
-    exists (L `union` L0).
-    intros y ?.
-    repeat split.
-    + apply H1...
-    + rewrite_nil_concat.
-      eapply wf_typ_ignores_typ_bindings.
-      apply H13...
-    + trivial...
-  - Case "typing_sub".
-    eauto using (sub_transitivity T).
-Qed.
-
-(*
-Lemma typing_narrowing_typ : forall F z U V E e T,
-  sub E U V ->
-  typing (F ++ [(z, bind_typ V)] ++ E) e T ->
-  typing (F ++ [(z, bind_typ U)] ++ E) e T.
-Proof with simpl_env; eauto using wf_typ_narrowing_typ, wf_env_narrowing_typ.
-  intros * Sub Typ.
-  eremember (F ++ [(z, bind_typ V)] ++ E) as G.
-  generalize dependent F.
-  induction Typ; intros F EQ; subst.
-  - Case "typing_var_tvar".
-    binds_cases H0.
-    + apply typing_var_tvar.
-      * eauto using wf_env_narrowing_typ.
-      * apply binds_weaken_at_head.
-        apply binds_weaken_at_head.
-        eauto.
-        apply ok_from_wf_env, wf_env_strengthening with (F := F)...
-        apply ok_from_wf_env...
-    + inversion H1; subst.
-      apply typing_sub with (S := U)...
-      * rewrite_env (empty ++ (F ++ [(x, bind_typ U)]) ++ E).
-        assert (WfU : wf_typ_in E U) by applys sub_regular Sub.
-        inversion WfU; subst.
-        -- apply typing_var_tvar...
-        -- apply typing_sub with (S := typ_capt (`cset_fvar` x) P).
-           ++ apply typing_var with (C := C)...
-           ++ apply sub_capt...
-              ** eapply subcapt_var with (T := typ_capt C P)...
-                 simpl.
-                 rewrite_env (empty ++ (F ++ [(x, bind_typ (typ_capt C P))]) ++ E).
-                 eapply subcapt_reflexivity with (A := dom (empty ++ (F ++ [(x, bind_typ (typ_capt C P))]) ++ E)).
-                 eapply wf_cset_in_weakening...
-                 repeat rewrite dom_concat...
-                 clear; fsetdec.
-              ** rewrite_env (empty ++ (F ++ [(x, bind_typ (typ_capt C P))]) ++ E).
-                 eapply sub_pre_reflexivity with (Ap := dom E) (Am := dom E)...
-                 rewrite_env (empty ++ (F ++ [(x, bind_typ (typ_capt C P))]) ++ E).
-                 eapply wf_pretyp_weakening with (Ap := dom E) (Am := dom E)...
-                 all: clear; fsetdec.
-      * rewrite_env (empty ++ (F ++ [(x, bind_typ U)]) ++ E).
-        apply sub_weakening...
-    + apply typing_var_tvar...
-  - Case "typing_var".
-    binds_cases H0.
-    + apply typing_var with (C := C).
-      * eauto using wf_env_narrowing_typ.
-      * simpl in Fr0.
-        assert (x <> z) by (clear - Fr0; fsetdec); clear Fr0.
-        apply binds_tail... 
-    + inversion H1; subst; clear H1.
-      inversion Sub; subst.
-      * apply typing_sub with (S := X).
-        -- apply typing_var_tvar...
-        -- eapply sub_trans_tvar with (U := U0).
-           ++ apply binds_tail.
-              apply binds_tail.
-              apply H0.
-              simpl.
-              ** enough (X <> x) by fsetdec.
-                 intros eq; subst.
-                 assert (ok ([(x, bind_typ (typ_capt C P))] ++ E)).
-                 { apply wf_env_strengthening in H.
-                   apply ok_from_wf_env, H.
-                 }
-                 inversion H2; subst.
-                 assert (x `in`A dom E) by applys binds_In H0.
-                 apply (H7 H3).
-              ** assert (ok (F ++ E)).
-                 { assert (ok (F ++ [(x, bind_typ (typ_capt C P))] ++ E)) by applys ok_from_wf_env H.
-                   eapply ok_remove_mid, H2.
-                 }
-                 assert (X `in`A dom E) by applys binds_In H0.
-                 eapply tail_not_in_head with (E := E)...
-           ++ admit.
-      * apply typing_sub with (S := typ_capt (`cset_fvar` x) P1).
-        -- apply typing_var with (C := C1)...
-        -- apply sub_capt.
-           ++ apply subcapt_reflexivity with (A := dom (F ++ [(x, bind_typ (typ_capt C1 P1))] ++ E)).
-              ** apply wf_concrete_cset...
-                 --- intros z zIn.
-                     assert (z = x) by (clear - zIn; fsetdec); subst; clear zIn.
-                     exists (typ_capt C1 P1).
-                     apply bound_typ...
-                 --- clear; fsetdec.
-              ** clear; fsetdec.
-           ++ rewrite_env (empty ++ (F ++ [(x, bind_typ (typ_capt C1 P1))]) ++ E).
-              apply sub_pre_weakening...
-    + assert (WfU : wf_typ_in E U) by applys sub_regular Sub.
-      inversion WfU; subst.
-      * apply typing_sub with (S := typ_capt (`cset_fvar` x) P).
-        -- apply typing_var with (C := C)...
-        -- apply sub_capt...
-           ++ eapply subcapt_var with (T := typ_capt C P)...
-              simpl; simpl_env.
-              admit.
-           ++ rewrite_env (empty ++ (F ++ [(z, bind_typ X)]) ++ E).
-              eapply sub_pre_reflexivity with (Ap := dom (F ++ [(z, bind_typ X)] ++ E)) (Am := dom (F ++ [(z, bind_typ X)] ++ E))...
-              rewrite_env (F ++ empty) in H2.
-              apply binds_weaken with (F := [(z, bind_typ X)] ++ E) in H2.
-              simpl_env in H2.
-              eapply wf_env_narrowing_typ with (U := X) in H...
-              destruct (wf_capt_from_typing_var _ _ _ _ H H2).
-              unfold wf_pretyp_in in H4.
-              replace (dom F `u`A {z}A `u`A dom E) with (dom (F ++ [(z, bind_typ X)] ++ E)).
-              apply H4.
-              repeat rewrite dom_concat; simpl; clear; fsetdec.
-              apply ok_from_wf_env...
-              all: clear; fsetdec.
-      * apply typing_sub with (S := typ_capt (`cset_fvar` x) P0).
-        -- apply typing_var with (C := C0)...
-           apply binds_tail.
-           apply binds_head.
-           apply binds_singleton.
-  - Case "typing_abs".
-    pick fresh x and apply typing_abs.
-    rewrite_env (([(x, bind_typ V)] ++ F) ++ [(z, bind_typ P)] ++ E).
-    apply H0...
-  - Case "typing_tabs".
-    pick fresh X and apply typing_tabs.
-    rewrite_env (([(X, bind_sub V)] ++ F) ++ [(z, bind_typ P)] ++ E).
-    apply H0...
-  - Case "typing_tapp".
-    apply typing_tapp with (T1 := T1).
-    apply IHe_T...
-    apply sub_specializing with (Q := Q)...
-  - Case "typing_let".
-    pick fresh x and apply typing_let...
-    rewrite_env (([(x, bind_typ T1)] ++ F) ++ [(z, bind_typ P)] ++ E).
-    apply H0...
-  - Case "typing_sub".
-    apply typing_sub with (S := S)...
-    apply sub_specializing with (Q := Q)...
-Qed.
-*)
-
-(*
-Lemma eval_typing_sub : forall E K S T U,
-  sub E S T ->
-  eval_typing E K T U ->
-  eval_typing E K S U.
-Proof with eauto*.
-  intros *.
-  intros Sub EvalTyp.
-  generalize dependent S.
-  induction EvalTyp; intros S Sub.
-  - apply typing_eval_nil...
-    apply sub_transitivity with (Q := T)...
-  - eapply typing_eval_cons with (L := L) (U := U)...
-    intros x x_fresh.
-    rewrite_env (empty ++ [(x, bind_typ S)] ++ E).
-    eapply typing_narrowing_typ_aux...
-    admit.
-Admitted.
-*)
-(*
-Lemma typing_arrow_inversion : forall E f C T1 T2,
-  typing E f (typ_capt C (typ_arrow T1 T2)) ->
-  exists U e L,
-    True. *)
-
-Tactic Notation "destructs" constr(E) :=
-  destruct ltac:(applys E).
-Tactic Notation "destructs" constr(E) "as" simple_intropattern(P) :=
-  destruct ltac:(applys E) as P.
-Tactic Notation "destructs" constr(E0) constr(A1) :=
-  destructs (>> E0 A1).
-Tactic Notation "destructs" constr(E0) constr(A1) "as" simple_intropattern(P) :=
-  destructs (>> E0 A1) as P.
-Tactic Notation "destructs" constr(E0) constr(A1) constr(A2) :=
-  destructs (>> E0 A1 A2).
-Tactic Notation "destructs" constr(E0) constr(A1) constr(A2) "as" simple_intropattern(P) :=
-  destructs (>> E0 A1 A2) as P.
-Tactic Notation "destructs" constr(E0) constr(A1) constr(A2) constr(A3) :=
-  destructs (>> E0 A1 A2 A3).
-Tactic Notation "destructs" constr(E0) constr(A1) constr(A2) constr(A3) "as" simple_intropattern(P) :=
-  destructs (>> E0 A1 A2 A3) as P.
-Tactic Notation "destructs" constr(E0) constr(A1) constr(A2) constr(A3) constr(A4) "as" simple_intropattern(P) :=
-  destructs (>> E0 A1 A2 A3 A4) as P.
-Tactic Notation "destructs" constr(E0) constr(A1) constr(A2) constr(A3) constr(A4) constr(A5) "as" simple_intropattern(P) :=
-  destructs (>> E0 A1 A2 A3 A4 A5) as P.
-Tactic Notation "destructs" constr(E0) constr(A1) constr(A2) constr(A3) constr(A4) constr(A5) constr(A6) "as" simple_intropattern(P) :=
-  destructs (>> E0 A1 A2 A3 A4 A5 A6) as P.
-
-Lemma binds_sub_arrow_implies_store_abs' : forall S E C P T1 T2 f,
-  store_typing S E ->
-  binds f (bind_typ (typ_capt C P)) E ->
-  f `~in`A (fv_ct T1 `u`A fv_ct T2) ->
-  sub_pre E P (typ_arrow T1 T2) ->
-  exists U e (abs_value : value (exp_abs U e)), stores S f (exp_abs U e) abs_value /\ sub E T1 U.
-Proof with eauto*.
-  intros * StoreTyp fBinds NotIn Sub.
-  induction StoreTyp; inversion fBinds; subst.
-  destruct (f == x).
-  - inversion H2; subst; clear H2.
-    unfold stores.
-    unfold binds.
-    simpl.
-    destruct (x == x); [ clear e | contradict n; reflexivity ].
-    inversion v_value; subst.
-    + inversion H; subst.
-      * exists T, e1, v_value.
-        inversion Sub; subst.
-        split...
-      * exists T, e1, v_value.
-        split...
-        rewrite_env (empty ++ [(x, bind_typ (typ_capt C P))] ++ E).
-        apply sub_weakening.
-        -- assert (Typ : typing E (exp_abs T e1) (typ_capt C (typ_arrow T1 T2))).
-           { apply typing_sub with (S := typ_capt C P)...
-             rewrite_env (empty ++ [(x, bind_typ (typ_capt C P))] ++ E) in Sub.
-             apply sub_pre_strengthening in Sub.
-             - apply sub_capt...
-               apply subcapt_reflexivity with (A := dom E)...
-             - simpl.
-               repeat apply notin_union...
-               destruct (sub_regular _ _ _ H3) as [_ [_ WfTyp]].
-               eapply wf_pretyp_in_notin_fv_cpt...
-           }
-           applys typing_abs_typ_arrow_implies_sub_param Typ.
-        -- apply wf_env_typ...
-    + assert (Typ : typing E (exp_tabs T e1) (typ_capt C (typ_arrow T1 T2))).
-      { apply typing_sub with (S := typ_capt C P)...
-        rewrite_env (empty ++ [(x, bind_typ (typ_capt C P))] ++ E) in Sub.
-        apply sub_pre_strengthening in Sub.
-        - apply sub_capt...
-          apply subcapt_reflexivity with (A := dom E)...
-        - destruct (sub_pre_regular _ _ _ Sub) as [WfEnv [WfTFun WfS]].
-          simpl.
-          repeat apply notin_union...
-          inversion WfEnv; inversion H6; subst.
-          eapply wf_pretyp_in_notin_fv_cpt...
-      }
-      exfalso.
-      destructs typing_regular Typ as [WfEnv [_ WfArr]].
-      clear - WfEnv WfArr Typ.
-      eremember (exp_tabs T e1) as abs.
-      eremember (typ_capt C (typ_arrow T1 T2)) as arr.
-      assert (Sub : sub E arr (typ_capt C (typ_arrow T1 T2))) by (subst; apply sub_reflexivity with (Ap := dom E) (Am := dom E); eauto* ).
-      clear Heqarr.
-      induction Typ; inversion Heqabs; subst.
-      inversion Sub; inversion H9.
-      apply IHTyp...
-      apply sub_transitivity with (Q := T0)...
-  - assert (Sub' : sub_pre E P (typ_arrow T1 T2)).
-    { rewrite_env (empty ++ [(x, bind_typ T)] ++ E) in Sub.
-      apply sub_pre_strengthening in Sub.
-      - apply Sub.
-      - repeat apply notin_union.
-        + fsetdec.
-        + apply wf_pretyp_in_notin_fv_cpt with (E := E)...
-          enough (WfCP : wf_typ_in E (typ_capt C P)) by (inversion WfCP; eauto* ).
-          apply wf_env_bound_implies_wf_typ with (x := f)...
-        + fold fv_ct.
-          admit.
-        + fold fv_ct.
-          admit.
-    }
-    destruct IHStoreTyp as [U [e [abs_value [xv_S_stores_f T1_sub_U]]]]...
-    exists U, e, abs_value.
-    split.
-    + rewrite_env ([(x, store v v_value)] ++ S).
-      apply binds_tail.
-      * trivial.
-      * simpl; fsetdec.
-    + rewrite_env (empty ++ [(x, bind_typ T)] ++ E).
-      apply sub_weakening...
-Admitted.
-
 Lemma subst_vv_open_vv : forall x u k y v,
   y <> x ->
   subst_vv x u (open_vv k y v) = open_vv k y (subst_vv x u v).
@@ -1862,281 +631,7 @@ Proof with auto using subst_vv_open_vv, subst_ct_open_ct_rec.
   intros * Neq Capt.
   revert k.
   induction e; intros k; simpl; f_equal...
-  Check subst_cset_open_cset_rec.
-  Check subst_ct_open_ct_rec.
   admit.
-  admit.
-  admit.
-Admitted.
-
-(*
-Lemma subcapt_through_subst_ct : forall E S1 C1 C2 x y,
-  wf_env E ->
-  y `~in`A dom E ->
-  binds x (bind_typ S1) E ->
-  subcapt E (open_cset 0 (`cset_fvar` x) C1) C2 ->
-  subcapt ([(y, bind_typ S1)] ++ E) (open_cset 0 (`cset_fvar` y) C1) C2.
-Proof with eauto*.
-  intros * WfEnv NotIn Binds Subcapt.
-  dependent induction Subcapt.
-  - Case "subcapt_universal".
-    apply subcapt_universal.
-    + rewrite_env (empty ++ [(y, bind_typ S1)] ++ E).
-      apply wf_cset_in_weakening...
-      apply ok_cons...
-    + inversion H0; subst.
-      unfold open_cset in H1 |- *.
-      dependent induction C1; simpl in *; simpl_env.
-      destruct_set_mem 0 t0.
-      * rewrite cset_concrete_union in H1 |- *.
-        inversion H1; subst.
-        assert (t0 `c`N {0}N).
-        { clear - OIn H6.
-          intros k kIn.
-          destruct (k === 0); subst.
-          - clear; fsetdec.
-          - assert (k `in`N ({}N `u`N t0 `\`N 0)).
-            { apply NatSet.F.union_3.
-              apply NatSet.F.remove_2...
-            }
-            rewrite <- H6 in H.
-            exfalso.
-            clear - H.
-            destruct (NatSetProperties.Dec.F.empty_iff k)...
-        }
-        clear H6.
-        econstructor.
-        -- intros z zIn.
-           destructs AtomSet.F.union_1 zIn.
-           ++ assert (z = y) by (clear - H4; fsetdec); subst...
-           ++ destruct (H2 z ltac:(fsetdec)) as [T [Bound | Bound]].
-              ** exists T.
-                 apply bound_typ, binds_tail...
-                 simpl.
-                 fsetdec.
-              ** exists T.
-                 apply bound_sub, binds_tail...
-                 simpl.
-                 fsetdec.
-        -- simpl.
-           fsetdec.
-      * rewrite <- H1.
-        rewrite_env (empty ++ [(y, bind_typ S1)] ++ E).
-        apply wf_cset_in_weakening...
-        apply ok_cons...
-  - Case "subcapt_in".
-    inversion H0; subst.
-    unfold open_cset in x |- *.
-    dependent induction C1; simpl in *; simpl_env.
-    destruct_set_mem 0 t0.
-    * rewrite cset_concrete_union in x |- *.
-      inversion x; subst.
-      simpl in x |- *; simpl_env.
-      assert (t0 `c`N {0}N).
-      { clear - OIn H4.
-        intros k kIn.
-        destruct (k === 0); subst.
-        - clear; fsetdec.
-        - assert (k `in`N ({}N `u`N t0 `\`N 0)).
-          { apply NatSet.F.union_3.
-            apply NatSet.F.remove_2...
-          }
-          rewrite <- H4 in H.
-          exfalso.
-          clear - H.
-          destruct (NatSetProperties.Dec.F.empty_iff k)...
-      }
-      clear H4.
-      constructor...
-      -- rewrite_env (empty ++ [(y, bind_typ S1)] ++ E).
-         apply wf_cset_in_weakening...
-         apply ok_cons...
-      -- intros z zIn.
-         destruct (AtomSetProperties.Dec.)
-         eapply subcapt_var. 
-
-
-
-Lemma sub_through_subst_ct : forall E S1 T2 x y U,
-  y `~in`A dom E ->
-  binds x (bind_typ S1) E ->
-  sub E (open_ct T2 (`cset_fvar` x)) U ->
-  sub ([(y, bind_typ S1)] ++ E) (open_ct T2 (`cset_fvar` y)) U
-with sub_pre_through_subst_cpt : forall E S1 P2 x y Q,
-  y `~in`A dom E ->
-  binds x (bind_typ S1) E ->
-  sub_pre E (open_cpt P2 (`cset_fvar` x)) Q ->
-  sub_pre ([(y, bind_typ S1)] ++ E) (open_cpt P2 (`cset_fvar` y)) Q.
-Proof with eauto*.
-{ intros * NotIn Binds Sub.
-  assert (WfEnv : wf_env E) by applys sub_regular Sub.
-  dependent induction Sub.
-  - Case "sub_refl_tvar".
-    unfold open_ct in x |- *.
-    induction T2; simpl in x |- *; simpl_env; subst...
-    inversion x; subst.
-    apply sub_refl_tvar.
-    + apply wf_env_typ...
-      apply wf_env_bound_implies_wf_typ with (x := x0)...
-    + rewrite_env (empty ++ [(y, bind_typ S1)] ++ E).
-      apply wf_typ_in_weakening...
-      apply ok_cons...
-  - Case "sub_trans_tvar".
-    unfold open_ct in x |- *.
-    induction T2; simpl in x |- *; simpl_env; subst...
-    inversion x; subst.
-    eapply sub_trans_tvar with (U := U).
-    + apply binds_tail...
-      simpl.
-      enough (a `in`A dom E) by fsetdec.
-      apply binds_In with (a := bind_sub U), H.
-    + rewrite_env (empty ++ [(y, bind_typ S1)] ++ E).
-      apply sub_weakening...
-      apply wf_env_typ...
-      apply wf_env_bound_implies_wf_typ with (x := x0)...
-  - Case "sub_capt".
-    unfold open_ct in x |- *.
-    induction T2; simpl in x |- *; simpl_env; subst...
-    inversion x; subst.
-    apply sub_capt.
-    + apply wf_env_typ...
-      apply wf_env_bound_implies_wf_typ with (x := x0)...
-    + rewrite_env (empty ++ [(y, bind_typ S1)] ++ E).
-      apply wf_typ_in_weakening...
-      apply ok_cons... 
-
-Lemma eval_typing_through_subst_ct : forall E K S1 T2 U x y,
-  y `~in`A dom E ->
-  binds x (bind_typ S1) E ->
-  eval_typing E K (open_ct T2 (`cset_fvar` x)) U ->
-  eval_typing ([(y, bind_typ S1)] ++ E) K (open_ct T2 (`cset_fvar` y)) U.
-Proof with eauto*.
-  intros * NotIn Binds EvalTyp.
-  assert (WfEnv : wf_env E) by applys eval_typing_regular EvalTyp.
-  dependent induction EvalTyp.
-  - Case "typing_eval_nil".
-    apply typing_eval_nil.
-    + apply wf_env_typ...
-      apply wf_env_bound_implies_wf_typ with (x := x)...
-    + rewrite_env ([(y, bind_typ S1)] ++ E).
-*)
-(*
-Lemma typing_through_subst_ve : forall U E F x T e u C,
-  typing (F ++ [(x, bind_typ U)] ++ E) e T ->
-  x `~in`A fv_cctx F ->
-  binds u (bind_typ U) E ->
-  typing (F ++ E) (subst_ve x u C e) T.
-Proof with simpl_env;
-           eauto 4 using wf_typ_strengthen,
-                         wf_env_strengthening,
-                         sub_strengthening.
-  intros * Typ NotIn uBinds.
-  eremember (F ++ [(x, bind_typ U)] ++ E) as E'.
-  generalize dependent F.
-  induction Typ; intros F EQ NotIn; subst; simpl subst_ve.
-  - Case "typing_var_tvar".
-    destruct (x0 == x); subst.
-    + SCase "x0 = x".
-      binds_get H0.
-      inversion H2; subst.
-      rewrite_env (empty ++ F ++ E).
-      apply typing_weakening...
-      apply wf_env_strengthening_typ in H...
-    + SCase "x0 <> x".
-      binds_cases H0.
-      eauto using wf_env_strengthening_typ.
-      eauto using wf_env_strengthening_typ.
-    - Case "typing_var".
-      destruct (x0 == x); subst.
-      + SCase "x0 = x".
-        binds_get H0.
-        inversion H2; subst; clear H2.
-        rewrite_env (empty ++ F ++ E).
-        apply typing_weakening...
-        apply wf_env_strengthening_typ in H...
-        admit.
-        admit.
-      + SCase "x0 <> x".
-        binds_cases H0.
-        admit.
-        admit.
-  - Case "typing_abs".
-    pick fresh y and apply typing_abs.
-    unfold open_ve.
-    rewrite subst_ve_open_ve_var...
-    rewrite <- concat_assoc.
-
-    (** Now we can apply the induction hypothesis. *)
-
-    apply H0...
-
-  (** The remaining cases in this proof are straightforward, given
-      everything that we have pointed out above. *)
-
-  Case "typing_app".
-    rewrite (if_hoist (f == x) u f var_f).
-    rewrite (if_hoist (x0 == x) u x0 var_f).
-    apply typing_app with (T1 := T1).
-    SCase "callee".
-      rewrite <- (if_hoist (f == x) u f var_f).
-      apply IHTypT1...
-    SCase "argument".
-      rewrite <- (if_hoist (x0 == x) u x0 var_f).
-      apply IHTypT2...
-
-  Case "typing_tabs".
-    pick fresh Y and apply typing_tabs.
-    rewrite subst_ve_open_te_var...
-    rewrite <- concat_assoc.
-    apply H0...
-
-  Case "typing_tapp".
-    rewrite (if_hoist (x0 == x) u x0 var_f).
-    apply typing_tapp with (T1 := T1).
-    SCase "callee".
-      rewrite <- (if_hoist (x0 == x) u x0 var_f).
-      apply IHTypT...
-    SCase "type argument".
-      eauto using sub_strengthening.
-
-  Case "typing_let".
-    pick fresh y and apply typing_let...
-    unfold open_ve.
-    rewrite subst_ve_open_ve_var...
-    rewrite <- concat_assoc.
-    apply H0...
-
-  Case "typing_pair".
-    rewrite (if_hoist (x1 == x) u x1 var_f).
-    rewrite (if_hoist (x2 == x) u x2 var_f).
-    apply typing_pair.
-    SCase "first element".
-      rewrite <- (if_hoist (x1 == x) u x1 var_f).
-      apply IHTypT1...
-    SCase "second element".
-      rewrite <- (if_hoist (x2 == x) u x2 var_f).
-      apply IHTypT2...
-
-  Case "typing_fst".
-    rewrite (if_hoist (x0 == x) u x0 var_f).
-    apply typing_fst with (T2 := T2).
-    rewrite <- (if_hoist (x0 == x) u x0 var_f).
-    apply IHTypT...
-
-  Case "typing_snd".
-    rewrite (if_hoist (x0 == x) u x0 var_f).
-    apply typing_snd with (T1 := T1).
-    rewrite <- (if_hoist (x0 == x) u x0 var_f).
-    apply IHTypT...
-Qed.
-*)
-
-Lemma eval_typing_open : forall E K T U V x y,
-  eval_typing E K (open_ct T (`cset_fvar` x)) U ->
-  eval_typing ([(y, bind_typ V)] ++ E) K (open_ct T (`cset_fvar` y)) U.
-Proof with eauto*.
-  intros * EvalTyp.
-  inversion EvalTyp; subst.
   admit.
   admit.
 Admitted.
@@ -2149,27 +644,6 @@ Proof with eauto*.
   induction StoreTyp...
   repeat rewrite dom_concat; simpl.
   rewrite IHStoreTyp...
-Qed.
-
-Lemma bound_notin_fv_cctx_implies_notin_ct : forall F x y T,
-  ok F ->
-  bound y T F ->
-  x `~in`A fv_cctx F ->
-  x `~in`A fv_ct T.
-Proof with eauto*.
-  intros * Ok Bound NotIn.
-  induction F; simpl in NotIn.
-  - inversion Bound; inversion H.
-  - destruct a as [z b].
-    replace ((z, b) :: F) with ([(z, b)] ++ F) in * by reflexivity.
-    destruct Bound as [Binds | Binds].
-    all: binds_cases Binds;
-         [ simpl in Fr;
-           inversion Ok; subst;
-           apply IHF; auto;
-           destruct b; fsetdec
-         | subst; fsetdec
-         ].
 Qed.
 
 Lemma subst_cset_cv_var_commutes_with_subst_vv : forall x u v,
@@ -2191,89 +665,6 @@ Proof with auto using subst_cset_cv_var_commutes_with_subst_vv.
   all: rewrite subst_cset_union;
        f_equal...
 Qed.
-
-(*
-Lemma wf_cset_through_subst_cset : forall F x u U E A C,
-  wf_env (F ++ [(x, bind_typ U)] ++ E) ->
-  wf_cset (F ++ [(x, bind_typ U)] ++ E) A C ->
-  binds u (bind_typ U) E ->
-  x `~in`A fv_cctx F ->
-  wf_cset (F ++ E) (A `\`A x) (subst_cset x (`cset_fvar` u) C).
-Proof with eauto*.
-  intros * WfEnv WfC Binds NotIn.
-  inversion WfC; subst.
-  unfold subst_cset.
-  destruct_set_mem x fvars; csetsimpl.
-  - destruct_set_mem u A.
-    + constructor.
-      * intros z zIn.
-        admit.
-      * enough (x <> u) by fsetdec.
-        admit.
-    + assert (x <> u).
-      { apply ok_from_wf_env in WfEnv as OkEnv.
-        apply binds_In in Binds.
-        enough (x `~in`A dom E) by fsetdec.
-        apply fresh_mid_tail in OkEnv...
-      }
-      apply wf_cset_strengthen_typ with (U := U).
-      * enough (x <> u) by fsetdec...
-      * constructor.
-        -- intros z zIn.
-           destruct_set_mem z fvars.
-           ++ apply (H z ltac:(fsetdec)).
-           ++ destruct (z == u); subst.
-              ** exists U...
-              ** exfalso; fsetdec.
-        -- intros z zIn.
-           destruct (z == u); subst.
-           ++  
-      replace ({u}A `u`A fvars `\`A x) with (({u}A `u`A fvars) `\`A x) by fsetdec.
-      
-      * 
-      * constructor. 
-
-Lemma wf_typ_through_subst_ct : forall F x u U E Ap Am T,
-  wf_env (F ++ [(x, bind_typ U)] ++ E) ->
-  wf_typ (F ++ [(x, bind_typ U)] ++ E) Ap Am T ->
-  binds u (bind_typ U) E ->
-  x `~in`A fv_cctx F ->
-  wf_typ (F ++ E) (Ap `\`A x) (Am `\`A x) (subst_ct x (`cset_fvar` u) T)
-with wf_pretyp_through_subst_cpt : forall F x u U E Ap Am P,
-  wf_env (F ++ [(x, bind_typ U)] ++ E) ->
-  wf_pretyp (F ++ [(x, bind_typ U)] ++ E) Ap Am P ->
-  binds u (bind_typ U) E ->
-  x `~in`A fv_cctx F ->
-  wf_pretyp (F ++ E) (Ap `\`A x) (Am `\`A x) (subst_cpt x (`cset_fvar` u) P).
-Proof with eauto*.
-{ intros * WfEnv WfT Binds NotIn.
-  eremember (F ++ [(x, bind_typ U)] ++ E) as E'.
-  generalize dependent F.
-  induction WfT; intros F Eq NotIn; subst; simpl.
-  - binds_cases H.
-    + apply wf_typ_var with (U := U0)...
-      enough (X <> x) by fsetdec.
-      simpl in Fr0; clear - Fr0; fsetdec.
-    + apply wf_typ_var with (U := U0)...
-      enough (X <> x) by fsetdec.
-      apply binds_In in H2.
-      enough (x `~in`A dom F) by fsetdec.
-      apply ok_from_wf_env in WfEnv.
-      apply fresh_mid_head in WfEnv...
-  - apply wf_typ_capt...
-    + apply wf_cset_strengthen_typ with (U := U).
-      * unfold subst_cset.
-        destruct_set_mem x (`cset_fvars` C).
-        -- simpl.
-           enough (x <> u) by fsetdec.
-           apply binds_In in Binds.
-           enough (x `~in`A dom E) by fsetdec.
-           apply ok_from_wf_env in WfEnv.
-           apply fresh_mid_tail in WfEnv.
-           assumption.
-        -- apply xIn.
-      * 
-*)
 
 Lemma subst_ve_open_ve : forall (e : exp) (x y u : atom) (c1 c2 : cap),
   y <> x ->
@@ -2303,6 +694,41 @@ Proof with auto*.
   destruct_set_mem x (`cset_fvar` y)...
   fsetdec.
 Qed.
+
+Fixpoint type_size (T : typ) : nat :=
+  match T with
+  | typ_fvar _ => 1
+  | typ_bvar _ => 1
+  | typ_capt _ P => pretype_size P + 1 
+  end
+with pretype_size (P : pretyp) : nat :=
+  match P with
+  | typ_top => 1
+  | typ_arrow T1 T2 => type_size T1 + type_size T2 + 1
+  | typ_all T1 T2 => type_size T1 + type_size T2 + 1
+  end.
+
+Lemma self_application_impossible : forall E x T,
+  ~ typing E (exp_app x x) T.
+Proof with eauto*.
+  intros * Typ.
+  dependent induction Typ.
+  clear IHTyp1 IHTyp2.
+  dependent induction Typ1.
+  - dependent induction Typ2; subst.
+    + assert (bind_typ X = bind_typ (typ_capt C (typ_arrow X T2))) by applys binds_unique H2 H0.
+      inversion H3.
+    + assert (bind_typ (typ_capt C0 P) = bind_typ (typ_capt C (typ_arrow (typ_capt (`cset_fvar` x0) P) T2))) by applys binds_unique H2 H0.
+      inversion H3; subst...
+      assert (pretype_size P = pretype_size (typ_arrow (typ_capt (`cset_fvar` x0) P) T2)) by (f_equal; apply H6).
+      clear - H4.
+      contradict H4.
+      simpl.
+      lia.
+    + admit.
+  - admit.
+  - admit.
+Admitted.
 
 Lemma typing_through_subst_ve : forall F E x T U e (u : atom),
   typing (F ++ [(x, bind_typ U)] ++ E) e T ->
@@ -2469,7 +895,7 @@ Proof with hint.
       rewrite subst_ct_open_ct_var,
               subst_ve_open_ve_var...
   - Case "typing_app".
-    assert (Neq : x0 <> x) by admit.
+    assert (Neq: x0 <> x) by admit.
     rewrite <- subst_ct_open_ct_var.
     assert (Iff : (if f == x then var_f u else var_f f) = var_f (if f == x then u else f))
        by (destruct_if; reflexivity).
@@ -2484,9 +910,8 @@ Proof with hint.
     + simpl in IHTyp2.
       rewrite Ifx0 in IHTyp2.
       apply IHTyp2...
-    + destruct (x0 == x)...
-      contradict e.
-      apply Neq.
+    + destruct (x0 == x); subst...
+      contradict Neq; reflexivity.
     + apply Neq.
     + trivial.
   - Case "typing_let".
@@ -2624,260 +1049,417 @@ Proof with eauto*.
     + apply subcapt_transitivity with (C2 := D)...
 Qed.
 
-Lemma typing_through_open_ve : forall E x y U e T,
+Lemma typing_through_subst_ve_typing : forall F E x T U e (u : atom),
+  no_type_bindings E ->
+  typing (F ++ [(x, bind_typ U)] ++ E) e T ->
+  typing E u U ->
+  typing (map (subst_cb x (`cset_fvar` u)) F ++ E)
+         (subst_ve x u (`cset_fvar` u) e)
+         (subst_ct x (`cset_fvar` u) T).
+Local Ltac hint ::=
+  eauto 4 using wf_env_subst_cb, typing_cv, subst_ct_fresh, subst_cpt_fresh, wf_typ_from_binds_typ, notin_fv_wf_pretyp.
+Proof with hint.
+  intros * NTB Typ uTyp.
+  assert (Ok : ok (F ++ [(x, bind_typ U)] ++ E)) by (apply ok_from_wf_env; applys typing_regular Typ).
+  destruct (typing_var_inversion' _ _ _ NTB uTyp) as [D [Q [D' [Q' [Eq [QSubQ' [xSubD' uBinds]]]]]]]; subst.
+  eremember (F ++ [(x, bind_typ (typ_capt D' Q'))] ++ E) as E'.
+  generalize dependent F.
+  induction Typ; intros F Eq; subst; simpl.
+  - Case "typing_var_tvar".
+    destruct (x0 == x); subst.
+    + SCase "x0 = x".
+      binds_cases H0.
+      * clear - Fr0; simpl in Fr0; exfalso; fsetdec.
+      * apply binds_In in H2.
+        assert (x `~in`A dom F) by (eapply fresh_mid_head; eauto).
+        clear - H0 H2; fsetdec.
+    + SCase "x0 <> x".
+      binds_cases H0.
+      * assert (WfX : wf_typ_in E X) by (apply wf_env_bound_implies_wf_typ with (x := x0); auto).
+        inversion WfX; subst.
+        contradict H2.
+        apply NTB.
+      * assert (x0 <> u).
+        { intros eq; subst.
+          apply binds_In in uBinds.
+          apply binds_In in H2.
+          enough (u `~in`A dom F) by fsetdec.
+          eapply tail_not_in_head...
+          simpl.
+          fsetdec.
+        }
+        eapply typing_var_tvar...
+        apply binds_head.
+        replace (bind_typ X) with (subst_cb x (`cset_fvar` u) (bind_typ X))...
+  - Case "typing_var".
+    destruct (x0 == x); subst.
+    + SCase "x0 = x".
+      binds_cases H0.
+      * clear - Fr0; simpl in Fr0; exfalso; fsetdec.
+      * inversion H1; subst; clear H1 H0.
+        rewrite <- subst_cpt_fresh.
+        2: {
+          apply wf_pretyp_notin_fv_cpt with (E := E) (Ap := dom E) (Am := dom E)...
+          eapply fresh_mid_tail...
+        }
+        unfold subst_cset.
+        destruct_set_mem x {x}A.
+        2: clear - xIn; exfalso; fsetdec.
+        clear xIn.
+        replace ({x}A `\`A x) with {}A by fsetdec.
+        replace (`cset_fvar` u `u` {}) with (`cset_fvar` u) by csetdec.
+        apply typing_sub with (S := typ_capt (`cset_fvar` u) Q).
+        -- apply typing_var with (C := D)...
+        -- rewrite_env (empty ++ map (subst_cb x (`cset_fvar` u)) F ++ E).
+           apply sub_weakening...
+           2: eapply wf_env_subst_cb...
+           apply sub_capt...
+           apply subcapt_reflexivity with (A := dom E)...
+           fsetdec.
+      * apply binds_In in H2.
+        assert (x `~in`A dom F) by (eapply fresh_mid_head; eauto).
+        clear - H0 H2; fsetdec.
+    + SCase "x0 <> x".
+      binds_cases H0.
+      * rewrite <- subst_cset_fresh with (x := x) (C1 := `cset_fvar` x0) (C2 := `cset_fvar` u),
+                <- subst_cpt_fresh with (x := x) (t := P) (c := `cset_fvar` u).
+        -- apply typing_var with (C := C)...
+        -- apply wf_pretyp_in_notin_fv_cpt with (E := E).
+           ++ enough (WfCP : wf_typ_in E (typ_capt C P)) by (inversion WfCP; auto).
+               apply wf_env_bound_implies_wf_typ with (x := x0)...
+           ++ apply fresh_mid_tail with (F := F) (a := bind_typ (typ_capt D' Q')).
+              apply ok_from_wf_env, H.
+        -- clear - n; fsetdec.
+      * rewrite <- subst_cset_fresh with (x := x) (C1 := `cset_fvar` x0) (C2 := `cset_fvar` u)...
+        apply typing_var with (C := subst_cset x (`cset_fvar` u) C)...
+        apply binds_head.
+        replace (bind_typ (typ_capt (subst_cset x (`cset_fvar` u) C) (subst_cpt x (`cset_fvar` u) P))) with (subst_cb x (`cset_fvar` u) (bind_typ (typ_capt C P))) by reflexivity.
+        apply binds_map...
+  - Case "typing_abs".
+    assert (WfEnv : wf_env (F ++ [(x, bind_typ (typ_capt D' Q'))] ++ E)). {
+      pick fresh z for L.
+      pose proof (H1 z Fr).
+      enough (WfE' : wf_env ([(z, bind_typ V)] ++ F ++ [(x, bind_typ (typ_capt D' Q'))] ++ E)) by (inversion WfE'; auto).
+      applys typing_regular H3.
+    }
+    rewrite subst_cset_cv_commutes_with_susbt_ve.
+    pick fresh y and apply typing_abs.
+    + eapply wf_typ_in_subst_cset...
+    + specialize (H0 y ltac:(clear - Fr; fsetdec)).
+      assert (NotIn : x `~in`A dom F /\ x `~in`A dom E /\ x <> y).
+      { apply ok_from_wf_env in WfEnv as OkEnv.
+        repeat split.
+        - apply fresh_mid_head in OkEnv; apply OkEnv.
+        - apply fresh_mid_tail in OkEnv; apply OkEnv.
+        - clear - Fr; fsetdec. 
+      }
+      replace (dom (map (subst_cb x (`cset_fvar` u)) F ++ E))
+         with (dom (F ++ [(x, bind_typ (typ_capt D' Q'))] ++ E) `\`A x).
+      2: {
+        clear - NotIn.
+        repeat rewrite dom_concat.
+        rewrite dom_map.
+        simpl.
+        fsetdec.
+      }
+      replace ((dom (F ++ [(x, bind_typ (typ_capt D' Q'))] ++ E) `\`A x) `u`A {y}A)
+         with ((dom (F ++ [(x, bind_typ (typ_capt D' Q'))] ++ E) `u`A {y}A) `\`A x).
+      2: {
+        clear - NotIn.
+        repeat rewrite dom_concat.
+        simpl.
+        fsetdec.
+      }
+      replace ([(y, bind_typ (subst_ct x (`cset_fvar` u) V))] ++ map (subst_cb x (`cset_fvar` u)) F ++ E)
+         with (map (subst_cb x (`cset_fvar` u)) ([(y, bind_typ V)] ++ F) ++ E)
+         by reflexivity.
+      rewrite subst_ct_open_ct_var.
+      * apply wf_typ_subst_cb with (Q := typ_capt D' Q').
+        -- apply H0.
+        -- apply wf_cset_extra.
+           ++ eapply wf_cset_from_binds...
+           ++ clear; repeat rewrite dom_concat; fsetdec.
+        -- apply wf_cset_extra.
+           ++ eapply wf_cset_from_binds...
+           ++ clear; repeat rewrite dom_concat; fsetdec.
+        -- simpl; apply ok_cons...
+        -- apply ok_cons...
+      * auto using NotIn.
+      * trivial.
+    + assert (Ok' : ok ([(y, bind_typ V)] ++ F ++ [(x, bind_typ (typ_capt D' Q'))] ++ E)) by (apply ok_cons; auto).
+      specialize (H2 y ltac:(clear - Fr; fsetdec) Ok' ([(y, bind_typ V)] ++ F) ltac:(reflexivity)).
+      assert (NotIn : x `~in`A dom F /\ x `~in`A dom E /\ x <> y).
+      { apply ok_from_wf_env in WfEnv as OkEnv.
+        repeat split.
+        - apply fresh_mid_head in OkEnv; apply OkEnv.
+        - apply fresh_mid_tail in OkEnv; apply OkEnv.
+        - clear - Fr; fsetdec. 
+      }
+      replace ([(y, bind_typ (subst_ct x (`cset_fvar` u) V))] ++ map (subst_cb x (`cset_fvar` u)) F ++ E)
+         with (map (subst_cb x (`cset_fvar` u)) ([(y, bind_typ V)] ++ F) ++ E)
+         by reflexivity.
+      rewrite subst_ct_open_ct_var,
+              subst_ve_open_ve_var...
+  - Case "typing_app".
+    assert (DeMorganNeqBoth: ~ (x0 = x /\ x0 = f)).
+    { intros [eqx eqf]; subst.
+      assert (typing (F ++ [(f, bind_typ (typ_capt D' Q'))] ++ E) (exp_app f f) (open_ct T2 (`cset_fvar` f))).
+      { eapply typing_app... }
+      contradict H.
+      apply self_application_impossible.
+    }
+    assert (NeqBoth : x0 <> x \/ x0 <> f).
+    { destruct (x0 == x); subst... }
+    destruct NeqBoth as [Neq | Neq].
+    + assert (Iff : (if f == x then var_f u else var_f f) = var_f (if f == x then u else f))
+        by (destruct_if; reflexivity).
+      assert (Ifx0 : (if x0 == x then var_f u else var_f x0) = (var_f (if x0 == x then u else x0)))
+        by (destruct_if; reflexivity).
+      rewrite Iff, Ifx0.
+      rewrite <- subst_ct_open_ct_var.
+      replace (`cset_fvar` x0) with (`cset_fvar` (if x0 == x then u else x0)).
+      apply typing_app with (T1 := subst_ct x (`cset_fvar` u) T1) (Cf := subst_cset x (`cset_fvar` u) Cf).
+      * simpl in IHTyp1.
+        rewrite Iff in IHTyp1.
+        apply IHTyp1...
+      * simpl in IHTyp2.
+        rewrite Ifx0 in IHTyp2.
+        apply IHTyp2...
+      * destruct (x0 == x); subst...
+        contradict Neq; reflexivity.
+      * apply Neq.
+      * trivial.
+    + admit.
+  - Case "typing_let".
+    pick fresh y and apply typing_let.
+    + apply IHTyp...
+    + rewrite subst_ve_open_ve_var...
+      replace ([(y, bind_typ (subst_ct x (`cset_fvar` u) T1))] ++ map (subst_cb x (`cset_fvar` u)) F ++ E)
+         with (map (subst_cb x (`cset_fvar` u)) ([(y, bind_typ T1)] ++ F) ++ E)
+         by reflexivity.
+      apply H0...
+  - Case "typing_tabs".
+    assert (WfEnv : wf_env (F ++ [(x, bind_typ (typ_capt D' Q'))] ++ E)). {
+      pick fresh Z for L.
+      pose proof (H1 Z Fr).
+      enough (WfE' : wf_env ([(Z, bind_sub V)] ++ F ++ [(x, bind_typ (typ_capt D' Q'))] ++ E)) by (inversion WfE'; auto).
+      applys typing_regular H3.
+    }
+    rewrite subst_cset_cv_commutes_with_susbt_ve.
+    pick fresh Y and apply typing_tabs.
+    + eapply wf_typ_in_subst_cset...
+    + specialize (H0 Y ltac:(clear - Fr; fsetdec)).
+      assert (NotIn : x `~in`A dom F /\ x `~in`A dom E /\ x <> Y).
+      { apply ok_from_wf_env in WfEnv as OkEnv.
+        repeat split.
+        - apply fresh_mid_head in OkEnv; apply OkEnv.
+        - apply fresh_mid_tail in OkEnv; apply OkEnv.
+        - clear - Fr; fsetdec. 
+      }
+      replace (dom (map (subst_cb x (`cset_fvar` u)) F ++ E))
+        with (dom (F ++ [(x, bind_typ (typ_capt D' Q'))] ++ E) `\`A x).
+      2: {
+        clear - NotIn.
+        repeat rewrite dom_concat.
+        rewrite dom_map.
+        simpl.
+        fsetdec.
+      }
+      replace ((dom (F ++ [(x, bind_typ (typ_capt D' Q'))] ++ E) `\`A x) `u`A {Y}A)
+        with ((dom (F ++ [(x, bind_typ (typ_capt D' Q'))] ++ E) `u`A {Y}A) `\`A x).
+      2: {
+        clear - NotIn.
+        repeat rewrite dom_concat.
+        simpl.
+        fsetdec.
+      }
+      replace ([(Y, bind_sub (subst_ct x (`cset_fvar` u) V))] ++ map (subst_cb x (`cset_fvar` u)) F ++ E)
+        with (map (subst_cb x (`cset_fvar` u)) ([(Y, bind_sub V)] ++ F) ++ E)
+        by reflexivity.
+      rewrite subst_ct_open_tt_var.
+      * apply wf_typ_subst_cb with (Q := typ_capt D' Q').
+        -- apply H0.
+        -- apply wf_cset_extra.
+          ++ eapply wf_cset_from_binds...
+          ++ clear; repeat rewrite dom_concat; fsetdec.
+        -- apply wf_cset_extra.
+          ++ eapply wf_cset_from_binds...
+          ++ clear; repeat rewrite dom_concat; fsetdec.
+        -- simpl; apply ok_cons...
+        -- apply ok_cons...
+      * auto using NotIn.
+      * trivial.
+    + assert (Ok' : ok ([(Y, bind_sub V)] ++ F ++ [(x, bind_typ (typ_capt D' Q'))] ++ E)) by (apply ok_cons; auto).
+      specialize (H2 Y ltac:(clear - Fr; fsetdec) Ok' ([(Y, bind_sub V)] ++ F) ltac:(reflexivity)).
+      assert (NotIn : x `~in`A dom F /\ x `~in`A dom E /\ x <> Y).
+      { apply ok_from_wf_env in WfEnv as OkEnv.
+        repeat split.
+        - apply fresh_mid_head in OkEnv; apply OkEnv.
+        - apply fresh_mid_tail in OkEnv; apply OkEnv.
+        - clear - Fr; fsetdec. 
+      }
+      replace ([(Y, bind_sub (subst_ct x (`cset_fvar` u) V))] ++ map (subst_cb x (`cset_fvar` u)) F ++ E)
+        with (map (subst_cb x (`cset_fvar` u)) ([(Y, bind_sub V)] ++ F) ++ E)
+        by reflexivity.
+      rewrite subst_ct_open_tt_var,
+              subst_ve_open_te_var...
+  - Case "typing_tapp".
+    assert (Ifx0 : (if x0 == x then var_f u else var_f x0) = (var_f (if x0 == x then u else x0)))
+      by (destruct_if; reflexivity).
+    rewrite Ifx0.
+    rewrite subst_ct_open_tt.
+    apply typing_tapp with (T1 := subst_ct x (`cset_fvar` u) T1) (C := subst_cset x (`cset_fvar` u) C).
+    + rewrite <- Ifx0.
+      apply IHTyp...
+    + apply sub_through_subst_ct with (U := typ_capt D' Q')...
+    + trivial.
+    + eapply bind_typ_notin_fv_tt with (S := typ_capt D' Q') (E := F ++ [(x, bind_typ (typ_capt D' Q'))] ++ E)...
+  - Case "typing_sub".
+    apply typing_sub with (S := subst_ct x (`cset_fvar` u) S)...
+    apply sub_through_subst_ct with (U := typ_capt D' Q')...
+Admitted.
+
+Lemma typing_through_open_ve_typing : forall E (x y : atom) U e T,
+  no_type_bindings E ->
   y `~in`A (fv_ct T `u`A fv_ve e `u`A fv_ce e) ->
   typing ([(y, bind_typ U)] ++ E) (open_ve e y (`cset_fvar` y)) (open_ct T (`cset_fvar` y)) ->
-  binds x (bind_typ U) E ->
+  typing E x U ->
   typing E (open_ve e x (`cset_fvar` x)) (open_ct T (`cset_fvar` x)).
 Proof with eauto*.
-  intros * NotIn Typ Binds.
+  intros * NTB NotIn Typ xTyp.
   assert (WfEnv : wf_env ([(y, bind_typ U)] ++ E)) by applys typing_regular Typ.
   assert (Neq : x <> y).
   { inversion WfEnv; subst.
     enough (x `in`A dom E) by fsetdec.
-    apply binds_In in Binds...
+    clear - xTyp.
+    dependent induction xTyp.
+    - apply binds_In in H0...
+    - apply binds_In in H0...
+    - apply IHxTyp...  
   }
   rewrite_env (map (subst_cb y (`cset_fvar` x)) empty ++ E).
   replace (open_ve e x (`cset_fvar` x))
      with (subst_ve y x (`cset_fvar` x) (open_ve e y (`cset_fvar` y)))
      by (rewrite <- subst_ve_intro; auto).
-     replace (open_ct T (`cset_fvar` x))
+  replace (open_ct T (`cset_fvar` x))
      with (subst_ct y (`cset_fvar` x) (open_ct T (`cset_fvar` y)))
      by (rewrite <- subst_ct_intro; auto).
-  apply typing_through_subst_ve with (U := U)...
+  apply typing_through_subst_ve_typing with (U := U)...
 Qed.
 
-Lemma typing_inv_let : forall E e k T,
-  typing E (exp_let e k) T ->
-  exists U,
-       typing E e U
-    /\ exists L, forall x, x `~in`A L ->
-         typing ([(x, bind_typ U)] ++ E) (open_ve k x (`cset_fvar` x)) T.
-Proof with eauto*.
-  intros * Typ.
-  dependent induction Typ...
-  destruct (IHTyp e k ltac:(reflexivity)) as [U [eTyp [L kTyp]]].
-  exists U.
-  split...
-  exists (L `u`A dom E).
-  intros y NotIn.
-  specialize (kTyp y ltac:(clear - NotIn; fsetdec)).
-  apply typing_sub with (S := S)...
-  rewrite_env (empty ++ [(y, bind_typ U)] ++ E).
-  apply sub_weakening...
-  apply wf_env_typ...
-  applys typing_regular eTyp. 
-Qed.
-
-Lemma typing_inv_abs' : forall E U e C P,
+Lemma typing_through_open_te : forall E (Y : atom) e T P Q,
   no_type_bindings E ->
-  typing E (exp_abs U e) (typ_capt C P) ->
-  exists T1 T2,
-     sub_pre E (typ_arrow T1 T2) P
-  /\ sub E T1 U
-  /\ exists L, forall x, x `~in`A L ->
-        typing ([(x, bind_typ T1)] ++ E) (open_ve e x (`cset_fvar` x))
-          (open_ct T2 (`cset_fvar` x))
-     /\ wf_typ ([(x, bind_typ T1)] ++ E) (dom E `u`A {x}A) 
-          (dom E) (open_ct T2 (`cset_fvar` x))
-     /\ sub ([(x, bind_typ T1)] ++ E) (open_ct T2 (`cset_fvar` x))
-          (open_ct T2 (`cset_fvar` x)).
+  Y `~in`A (fv_tt T `u`A fv_ct T `u`A fv_te e `u`A fv_ce e) ->
+  typing ([(Y, bind_sub Q)] ++ E) (open_te e Y) (open_tt T Y) ->
+  sub E P Q ->
+  `cset_uvar` (cv P) <> true ->
+  typing E (open_te e P) (open_tt T P).
+Proof with eauto*.
+  intros * NTB NotIn Typ Sub NotUniv.
+  rewrite_env (map (subst_tb Y P) empty ++ E).
+  replace (open_te e P)
+     with (subst_te Y P (open_te e Y))
+     by (symmetry; apply subst_te_intro; clear - NotIn; fsetdec).
+  replace (open_tt T P)
+     with (subst_tt Y P (open_tt T Y))
+     by (symmetry; apply subst_tt_intro; clear - NotIn; fsetdec).
+  apply typing_through_subst_te with (Q := Q)...
+Qed.
+
+Lemma typing_inv_app : forall E (f x : atom) T,
+  no_type_bindings E ->
+  typing E (exp_app f x) T ->
+  exists C T1 T2, typing E f (typ_capt C (typ_arrow T1 T2))
+    /\ typing E x T1
+    /\ sub E (open_ct T2 (`cset_fvar` x)) T.
 Proof with eauto*.
   intros * NTB Typ.
-  assert (WfEnv : wf_env E) by applys typing_regular Typ.
-  dependent induction Typ.
-  - Case "typing_abs".
-    repeat eexists.
-    + apply sub_pre_reflexivity with (Ap := dom E) (Am := dom E)...
-    + apply sub_reflexivity with (Ap := dom E) (Am := dom E)...
-    + (* REVIEW: how to use instantiate? *)
-      Unshelve. 2: apply (L `u`A dom E).
-      apply (H1 x ltac:(clear - H3; fsetdec)).
-    + apply (H0 x ltac:(clear - H3; fsetdec)).
-    + apply sub_reflexivity with (Ap := dom ([(x, bind_typ U)] ++ E)) (Am := dom E)...
-      replace (dom ([(x, bind_typ U)] ++ E)) with (dom E `u`A {x}A) by (clear; simpl; fsetdec).
-      apply (H0 x ltac:(clear - H3; fsetdec)).
-      clear; simpl; fsetdec.
-  - Case "typing_sub".
-    destructs sub_left_capt_inversion NTB H as [D [Q Eq]].
-    destruct (IHTyp U e D Q NTB ltac:(reflexivity) Eq WfEnv) as [T1 [T2 [T1T2SubQ [T1SubU [L' ?]]]]].
-    exists T1, T2.
-    repeat split...
-    apply sub_pre_transitivity with (Q := Q).
-    + apply pretype_from_wf_pretyp with (E := E) (Ap := dom E) (Am := dom E)...
-      applys sub_pre_regular T1T2SubQ.
-    + apply T1T2SubQ.
-    + subst.
-      inversion H; subst...
-Qed.
-
-Lemma store_typing_regular : forall S E,
-  store_typing S E ->
-  wf_env E.
-Proof with eauto*.
-  intros * StoreTyp.
-  induction StoreTyp...
-  apply wf_env_typ...
-  applys typing_regular H.
-Qed.
-
-(*
-Lemma type_of_abs_is_capt_top_or_arrow : forall E U e T,
-  typing E (exp_abs U e) *)
-
-Lemma store_abs_inversion : forall E S f U e abs_value,
-  store_typing S E ->
-  stores S f (exp_abs U e) abs_value ->
-  exists C P T1 T2,
-     typing E (exp_abs U e) (typ_capt C P)
-  /\ sub_pre E (typ_arrow T1 T2) P
-  /\ sub E T1 U.
-Proof with eauto*.
-  intros * StoreTyp Stores.
-  induction StoreTyp; inversion Stores; subst; rename H into Typ, H0 into NotIn.
-  destruct (f == x); subst.
-  - Case "f = x".
-    clear IHStoreTyp.
-    inversion H2; subst; clear H2.
-    clear Stores.
-    assert (WfEnv : wf_env ([(x, bind_typ T)] ++ E)).
-    { apply wf_env_typ.
-      - applys typing_regular Typ.
-      - applys typing_regular Typ.
-      - apply NotIn.
-    }
-    destruct (values_have_precise_captures _ _ _ abs_value Typ) as [P [Typ' Sub']].
-    simpl in *; simpl_env in *.
-    destruct (sub_capt_inversion _ _ _ _ Sub') as [D [Q [Eq [CSubD PSubQ]]]]; subst.
-    assert (NTB : no_type_bindings E) by applys store_typing_no_type_bindings StoreTyp.
-    destruct (typing_inv_abs' E U e (free_for_cv e) P NTB Typ') as [T1 [T2 [T1T2SubP [T1SubU [L ?]]]]].
-    rewrite_env (empty ++ [(x, bind_typ (typ_capt D Q))] ++ E).
-    repeat eexists.
-    + apply typing_weakening... 
-    + apply sub_pre_weakening...
-    + apply sub_weakening...
-  - Case "f <> x".
-    destruct (IHStoreTyp H2) as [C [P [T1 [T2 [Typ' [T1T2SubP T1SubU]]]]]].
-    rewrite_env (empty ++ [(x, bind_typ T)] ++ E).
-    assert (WfT : wf_typ_in E T) by applys typing_regular Typ.
-    assert (WfEnv : wf_env ([(x, bind_typ T)] ++ E)) by (apply wf_env_typ; auto).
-    repeat eexists.
-    + apply typing_weakening...
-    + apply sub_pre_weakening...
-    + apply sub_weakening...
-Qed.
-
-Lemma sub_pre_arrow_inversion' : forall E P T1 T2,
-  sub_pre E P (typ_arrow T1 T2) ->
-  exists S1 S2, P = typ_arrow S1 S2
-             /\ sub E T1 S1
-             /\ exists L, forall x, x `~in`A L ->
-                    sub ([(x, bind_typ T1)] ++ E) (open_ct S2 (`cset_fvar` x)) (open_ct T2 (`cset_fvar` x)).
-Proof with eauto*.
-  intros * Sub.
-  dependent induction Sub.
-  exists S1, S2...
-Qed.
-
-Check typing_app.
-
-Lemma typing_inv_app : forall E (f x : atom) T2,
-  typing E (exp_app f x) T2 ->
-  exists C S1 S2, typing E f (typ_capt C (typ_arrow S1 S2))
-               /\ typing E x S1.
-Proof with eauto*.
-  intros * Typ.
   dependent induction Typ.
   - Case "typing_app".
-    clear IHTyp1 IHTyp2.
     exists Cf, T1, T2.
     repeat split...
-  - Case "typing_sub".
-    destruct (IHTyp f x ltac:(reflexivity)) as [C [S1 [S2 [fTyp xTyp]]]]...
+    destructs typing_regular Typ1 as [WfEnv [_ WfCfT1T2]].
+    inversion WfCfT1T2; subst.
+    inversion H5; subst.
+    apply sub_reflexivity with (Ap := dom E) (Am := dom E)...
+    pick fresh z and specialize H7.
+    replace (open_ct T2 (`cset_fvar` x))
+       with (subst_ct z (`cset_fvar` x) (open_ct T2 (`cset_fvar` z))).
+    replace (dom E) with (dom E `\`A z).
+    replace (wf_typ E (dom E `\`A z)) with (wf_typ E (dom ([(z, bind_typ T1)] ++ E) `\`A z)).
+    rewrite_env (map (subst_cb z (`cset_fvar` x)) empty ++ E).
+    eapply wf_typ_subst_cb with (Q := T1); csetsimpl...
+    + replace ({z}A `u`A dom E) with (dom E `u`A {z}A) by (clear; fsetdec).
+      apply H7.
+    + apply wf_cset_set_weakening with (A := dom E).
+      2: fsetdec.
+      destructs typing_var_inversion' NTB Typ2 as [C [P [_ [_ [_ [_ [_ Binds]]]]]]].
+      eapply wf_cset_from_binds...
+    + destructs typing_var_inversion' NTB Typ2 as [C [P [_ [_ [_ [_ [_ Binds]]]]]]].
+      eapply wf_cset_from_binds...
+    + f_equal.
+      simpl.
+      clear; fsetdec.
+    + assert (z `~in`A dom E) by (clear - Fr; fsetdec).
+      clear - H; fsetdec.
+    + symmetry.
+      apply subst_ct_intro.
+      clear - Fr; fsetdec.     
+  - destruct (IHTyp f x NTB eq_refl) as [C [T1 [T2 [fTyp [xTyp Seq]]]]].
+    exists C, T1, T2.
+    repeat split...
+    apply sub_transitivity with (Q := S)...
 Qed.
 
-(*
-Lemma red_app_inversion : forall S E f x e T1 T2 v (v_value : value v) (abs_value : value (exp_abs T1 e)),
-  store_typing S E ->
-  stores S f (exp_abs T1 e) abs_value ->
-  stores S x v v_value ->
-  typing E (exp_app f x) T2 ->
-     typing E v T1
-  /\ typing E (exp_abs T1 e) (typ_capt (free_for_cv e) (typ_arrow T1 T2)).
+Lemma typing_tapp_inversion : forall E (x : atom) U T,
+  no_type_bindings E ->
+  typing E (exp_tapp x U) T ->
+  exists C T1 T2, typing E x (typ_capt C (typ_all T1 T2))
+    /\ sub E U T1
+    /\ sub E (open_tt T2 U) T.
 Proof with eauto*.
-  intros * StoreTyp fStores xStores TypApp.
-  assert (NTB : no_type_bindings E) by applys store_typing_no_type_bindings StoreTyp.
-  dependent induction TypApp.
-  - clear IHTypApp1 IHTypApp2.
-    rename TypApp1 into fTyp, TypApp2 into xTyp.
-    rename Cf into C.
-    destructs typing_var_inversion' NTB fTyp as [Cf [Pf [Df [Qf [Eqf [PfSubQf fBinds]]]]]]; subst.
-    destructs typing_var_inversion' NTB xTyp as [Cx [Px [Dx [Qx [Eqx [PxSubQx xBinds]]]]]]; subst.
-    inversion Eqf; subst; clear Eqf.
-    destructs sub_pre_arrow_inversion' PfSubQf as [S1 [S2 [Eq [T1SubS1 [L ?]]]]]; subst.
-    destructs stores_preserves_typing StoreTyp xStores xTyp as [Rx [vTyp RxSubQx]].
-    destructs stores_preserves_typing StoreTyp fStores fTyp as [Rf [absTyp RfSubQf]].
-    simpl in *; simpl_env in *.
-    destructs sub_pre_arrow_inversion' RfSubQf as [R1 [R2 [Eq [DQSubR1 [L' ?]]]]]; subst.
-    assert (sub E (typ_capt (free_for_cv e) (typ_arrow R1 R2))
-                  (typ_capt (free_for_cv e) (typ_arrow (typ_capt Dx Qx) R2))).
-    { apply sub_capt.
-      - apply subcapt_reflexivity with (A := dom E)...
-      - inversion RfSubQf; subst.
-        apply sub_arrow with (L := L0 `u`A dom E)...
-        + intros z zIn.
-          specialize (H10 z ltac:(clear - zIn; fsetdec)).
-          rewrite_env (empty ++ [(z, bind_typ (typ_capt Dx Qx))] ++ E).
-          eapply wf_typ_narrowing_typ_base with (V := R1)...
-          apply ok_cons...
-        + intros z zIn.
-          apply sub_reflexivity with (Ap := dom ([(z, bind_typ (typ_capt Dx Qx))] ++ E)) (Am := dom ([(z, bind_typ (typ_capt Dx Qx))] ++ E))...
-          specialize (H11 z ltac:(clear - zIn; fsetdec)).
-          applys sub_regular H11.
+  intros * NTB Typ.
+  dependent induction Typ.
+  - Case "typing_tapp".
+    exists C, T1, T2.
+    repeat split...
+    destructs typing_regular Typ as [WfEnv [_ WfCT1T2]].
+    inversion WfCT1T2; subst.
+    inversion H6; subst.
+    apply sub_reflexivity with (Ap := dom E) (Am := dom E)...
+    pick fresh Z and specialize H8.
+    replace (open_tt T2 U)
+       with (subst_tt Z U (open_tt T2 Z)).
+    replace (dom E) with (dom ([(Z, bind_sub T1)] ++ E) `\`A Z).
+    rewrite_env (map (subst_tb Z U) empty ++ E).
+    assert (WfU : wf_typ E ({Z}A `u`A dom E) ({Z}A `u`A dom E) U).
+    { rewrite_env (empty ++ empty ++ E).
+      eapply wf_typ_weakening with (Ap := dom E) (Am := dom E)...
+      applys sub_regular H.
+      all: simpl; clear; fsetdec.
     }
-    destruct (typing_inv_abs _ _ _ _ absTyp (typ_capt Dx Qx) R2 (free_for_cv e) H1) as [DxQxSubT1 [Q2 [L'' ?]]].
-    split.
-    + apply typing_sub with (S := typ_capt (free_for_cv v) Rx)...
-      apply sub_transitivity with (Q := typ_capt Dx Qx)...
-      apply sub_capt...
-      admit.
-    +   
-*)
-
-Inductive red : state -> state -> Prop :=
-  | red_lift : forall x v (v_value : value v) k (k_scope : scope k) S K,
-      x `~in`A dom S ->
-      red ⟨ S | cont k k_scope :: K | v ⟩
-          ⟨ [(x, store v v_value)] ++ S | K | open_ve k x (`cset_fvar` x) ⟩
-  | red_let_var : forall (x y : atom) v (v_value : value v) k (k_scope : scope k) S K,
-      stores S x v v_value ->
-      red ⟨ S | cont k k_scope :: K | x ⟩
-          ⟨ S | K | open_ve k x (`cset_fvar` x) ⟩
-  | red_let_val : forall x v (v_value : value v) k (k_scope : scope k) S K,
-      x `~in`A dom S ->
-      red ⟨ S | K | exp_let v k ⟩
-          ⟨ [(x, store v v_value)] ++ S | K | open_ve k x (`cset_fvar` x) ⟩
-  | red_let_exp : forall e k (k_scope : scope k) S K,
-      red ⟨ S | K | exp_let e k ⟩
-          ⟨ S | cont k k_scope :: K | e ⟩
-  | red_app : forall f x y U e v (v_value : value v) (abs_value : value (exp_abs U e)) S K,
-      stores S f (exp_abs U e) abs_value ->
-      stores S x v v_value ->
-      y `~in`A dom S ->
-      red ⟨ S | K | exp_app f x ⟩
-          ⟨ [(y, store v v_value)] ++ S | K | open_ve e y (`cset_fvar` y) ⟩
-  | red_tapp : forall x T U e (tabs_value : value (exp_tabs U e)) S K,
-      stores S x (exp_tabs U e) tabs_value ->
-      type T ->
-      red ⟨ S | K | exp_tapp x T ⟩
-          ⟨ S | K | open_te e T ⟩.
+    eapply wf_typ_subst_tb with (Q := T1); csetsimpl...
+    + replace ({Z}A `u`A dom E) with (dom E `u`A {Z}A) by (clear; fsetdec).
+      apply H8.
+    + simpl.
+      assert (Z `~in`A dom E) by (clear - Fr; fsetdec).
+      clear - H0.
+      fsetdec.
+    + symmetry.
+      apply subst_tt_intro.
+      clear - Fr; fsetdec.     
+  - destruct (IHTyp x U NTB eq_refl) as [C [T1 [T2 [fTyp [xTyp Seq]]]]].
+    exists C, T1, T2.
+    repeat split...
+    apply sub_transitivity with (Q := S)...
+Qed.
 
 Lemma preservation : forall s s' V,
   state_typing s V ->
   red s s' ->
   state_typing s' V.
 Ltac hint :=
-    eauto using wf_cset_set_weakening.
+    eauto using wf_cset_set_weakening, no_type_bindings_cons.
 Proof with hint.
   intros * [S K e E T U StoreTyp EvalTyp Typ] Red.
   assert (WfEnv : wf_env E) by applys eval_typing_regular EvalTyp.
@@ -2898,7 +1480,8 @@ Proof with hint.
         applys eval_typing_regular H6.
       }
       rewrite open_ct_rec_type with (k := 0) (C := `cset_fvar` x)...
-      apply typing_through_open_ve with (y := y) (U := T).
+      apply typing_through_open_ve_typing with (y := y) (U := T).
+      * apply no_type_bindings_cons...
       * clear - Fr; fsetdec.
       * apply typing_weakening.
         unfold open_ct.
@@ -2913,598 +1496,316 @@ Proof with hint.
            apply wf_typ_in_weakening...
            apply ok_cons...
         -- rewrite dom_concat; simpl; clear - Fr; fsetdec.
-      * apply binds_head...
+      * destruct T.
+        -- apply typing_sub with (S := typ_capt (`cset_fvar` x) p).
+           ++ eapply typing_var...
+           ++ assert (Wfcp : wf_typ_in E (typ_capt c p)) by applys typing_regular Typ.
+              inversion Wfcp; subst.
+              apply sub_capt...
+              ** eapply subcapt_var...
+                 cbn [cv].
+                 apply subcapt_reflexivity with (A := dom ([(x, bind_typ (typ_capt c p))] ++ E)).
+                 2: fsetdec.
+                 rewrite_env (empty ++ [(x, bind_typ (typ_capt c p))] ++ E).
+                 apply wf_cset_in_weakening...
+                 apply ok_cons...
+              ** apply sub_pre_reflexivity with (Ap := dom ([(x, bind_typ (typ_capt c p))] ++ E)) (Am := dom ([(x, bind_typ (typ_capt c p))] ++ E))...
+                 2,3: fsetdec.
+                 rewrite_env (empty ++ [(x, bind_typ (typ_capt c p))] ++ E).
+                 apply wf_pretyp_in_weakening...
+                 apply ok_cons...
+        -- enough (Wfn : wf_typ_in E n) by inversion Wfn.
+           applys typing_regular Typ.
+        -- assert (Wfa : wf_typ_in E a) by applys typing_regular Typ.
+           inversion Wfa; subst.
+           contradict H3.
+           apply NTB. 
   - Case "red_let_var".
     inversion EvalTyp; subst.
-    destructs typing_var_inversion' NTB Typ as [C [P [D [Q [Eq [PSubQ [xSubD Binds]]]]]]]; subst.
-    destructs stores_preserves_typing StoreTyp H Typ as [B [R [vTyp [Binds' [vSubB RSubQ]]]]].
-    assert (bind_typ (typ_capt B R) = bind_typ (typ_capt C P)) by applys binds_unique Binds' Binds.
-    inversion H1; subst; clear H1.
     eapply typing_state with (E := E) (T := U0)...
+    pick fresh z and specialize H5.
     assert (type_U0 : type U0).
     { enough (WfU : wf_typ_in E U0) by applys type_from_wf_typ WfU.
       applys eval_typing_regular H6.
     }
     rewrite open_ct_rec_type with (k := 0) (C := `cset_fvar` x)...
-    apply typing_through_open_ve with (y := y) (U := typ_capt C P)...
+    apply typing_through_open_ve_typing with (y := z) (U := T)...
+    destructs typing_var_inversion' NTB Typ as [C [P [D [Q [Eq [PSubQ [xSubD Binds]]]]]]]; subst.
+    destructs stores_preserves_typing StoreTyp H Typ as [B [R [vTyp [Binds' [vSubB RSubQ]]]]].
+    assert (bind_typ (typ_capt B R) = bind_typ (typ_capt C P)) by applys binds_unique Binds' Binds.
+    inversion H0; subst; clear H0.
     unfold open_ct.
     rewrite <- open_ct_rec_type...
-    apply typing_weakening.
-    rewrite_env (empty ++ [(z, bind_typ (typ_capt C P))] ++ E).
-    apply typing_narrowing_typ with (Q := typ_capt D Q)...
-    apply sub_capt...
-    admit.
-    destructs typing_var_inversion' NTB Typ as [C [P [D [Q [Eq [PSubQ Binds]]]]]]; subst.
   - Case "red_let_val".
     assert (x `~in`A dom E) by (rewrite <- (store_typing_preserves_dom _ _ StoreTyp); assumption).
     destructs typing_inv_let Typ as [T1 [eTyp [L kTyp]]].
     eapply typing_state with (E := [(x, bind_typ T1)] ++ E) (T := T).
-    * apply typing_store_cons...
-    * rewrite_env (empty ++ [(x, bind_typ T1)] ++ E).
+    + apply typing_store_cons...
+    + rewrite_env (empty ++ [(x, bind_typ T1)] ++ E).
       apply eval_typing_weakening...
       apply wf_env_typ...
       applys typing_regular eTyp.
-    * pick fresh z and specialize kTyp.
+    + pick fresh z and specialize kTyp.
       assert (type_T : type T).
       { enough (WfT : wf_typ_in E T) by applys type_from_wf_typ WfT.
         applys typing_regular Typ.
       }
       rewrite open_ct_rec_type with (k := 0) (C := `cset_fvar` x)...
-      eapply typing_through_open_ve with (y := z) (U := T1)...
-      apply typing_weakening.
-      unfold open_ct.
-      rewrite <- open_ct_rec_type...
-      assert (WfT1 : wf_typ_in E T1) by applys typing_regular eTyp.
-      repeat apply wf_env_typ...
-      rewrite_env (empty ++ [(x, bind_typ T1)] ++ E).
-      apply wf_typ_in_weakening...
-      apply ok_cons...
+      eapply typing_through_open_ve_typing with (y := z) (U := T1)...
+      * apply typing_weakening.
+        unfold open_ct.
+        rewrite <- open_ct_rec_type...
+        assert (WfT1 : wf_typ_in E T1) by applys typing_regular eTyp.
+        repeat apply wf_env_typ...
+        rewrite_env (empty ++ [(x, bind_typ T1)] ++ E).
+        apply wf_typ_in_weakening...
+        apply ok_cons...
+      * assert (wf_typ_in E T1) by applys typing_regular eTyp.
+        inversion H1; subst.
+        -- contradict H2; apply NTB.
+        -- apply typing_sub with (S := typ_capt (`cset_fvar` x) P)...
+           apply sub_capt.
+           ++ eapply subcapt_var...
+              cbn [cv].
+              rewrite_env (empty ++ [(x, bind_typ (typ_capt C P))] ++ E).
+              apply subcapt_weakening.
+              2: apply wf_env_typ...
+              apply subcapt_reflexivity with (A := dom E)...
+              clear; fsetdec.
+           ++ rewrite_env (empty ++ [(x, bind_typ (typ_capt C P))] ++ E).
+              apply sub_pre_weakening.
+              2: apply wf_env_typ...
+              apply sub_pre_reflexivity with (Ap := dom E) (Am := dom E)...
+              all: clear; fsetdec. 
   - Case "red_let_exp".
     destructs typing_inv_let Typ as [T1 [eTyp [L kTyp]]].
     eapply typing_state with (E := E) (T := T1)...
     eapply typing_eval_cons...
   - Case "red_app".
-    destructs stores_preserves_typing
-    eapply typing_state with (E := )
-
-    eapply typing_state with (E := E) (T := T)...
-    destructs store_abs_inversion StoreTyp H as [C [P [T1 [T2 [TypAbs [T1T2SubP T1SubU]]]]]].
-    destructs typing_inv_abs' NTB TypAbs as [S1 [S2 [S1S2SubP [S1SubU0 [L ?]]]]].
-    pick fresh z and specialize H1.
-    destruct H1 as [eTyp [WfS2 Sub]].
-    assert (type_T : type T).
-    { enough (WfT : wf_typ_in E T) by applys type_from_wf_typ WfT.
-      applys typing_regular Typ.
-    }
-    rewrite open_ct_rec_type with (k := 0) (C := `cset_fvar` x)...
-    eapply typing_through_open_ve with (y := z) (U := S1)...
-    eapply binds_fresh.
-    admit.
-    destruct (P2 x) as [? ?]...
-    rewrite (subst_ee_intro x)...
-    rewrite_env (empty ++ E).
-    apply (typing_through_subst_ee T).
-      apply (typing_sub S2)...
-        rewrite_env (empty ++ [(x, bind_typ T)] ++ E).
-        apply sub_weakening...
-      eauto.
-    
-
-
-  induction Typ.
-  - Case "typing_var".
-    inversion EvalTyp; subst.
-    + SCase "typing_eval_nil".
-      specialize (Red {}A); inversion Red; subst; inversion v_value.
-    + SCase "typing_eval_cons".
-      specialize (Red (dom E `u`A L)); inversion Red; subst.
-      * SSCase "red_lift".
-        inversion v_value.
-      * SSCase "red_let_var".
-        apply typing_state with (E := E) (T := U0)...
-        -- apply typing_store_cons...
-           eapply stores_preserves_typing...
-        -- rewrite_env (empty ++ [(y, bind_typ X)] ++ E).
-           apply eval_typing_weakening...
-           apply wf_env_typ...
-           destruct (typing_regular _ _ _ (H1 y (ltac:(fsetdec)))) as [wf_xT_Γ _].
-           inversion wf_xT_Γ; subst...
-  - Case "typing_capt".
-    inversion EvalTyp; subst.
-    + SCase "typing_eval_nil".
-      specialize (Red {}A); inversion Red; subst; inversion v_value.
-    + SCase "typing_eval_cons".
-      specialize (Red (dom E `u`A L)); inversion Red; subst.
-      * SSCase "red_lift".
-        inversion v_value.
-      * SSCase "red_let_var".
-        destructs wf_capt_from_typing_var H H0 as [WfC WfP]...
-        apply typing_state with (E := [(y, bind_typ (typ_capt (`cset_fvar` x) P))] ++ E) (T := U0).
-        -- apply typing_store_cons...
-           eapply stores_preserves_typing...
-        -- rewrite_env (empty ++ [(y, bind_typ (typ_capt (`cset_fvar` x) P))] ++ E).
-           apply eval_typing_weakening...
-           apply wf_env_typ...
-           constructor...
-           constructor...
-           ++ intros z zIn; assert (z = x) by (clear - zIn; fsetdec); subst; clear zIn...
-           ++ enough (x `in`A dom E) by fsetdec.
-              apply binds_In with (a := bind_typ (typ_capt C P))... 
-        -- rewrite_env (empty ++ [(y, bind_typ (typ_capt (`cset_fvar` x) P))] ++ E).
-           specialize (H1 y ltac:(fsetdec)).
-           apply H1.
-  - Case "typing_abs".
-    inversion EvalTyp; subst.
-    + SCase "typing_eval_nil".
-      specialize (Red {}A); inversion Red.
-    + SCase "typing_eval_cons".
-      specialize (Red (dom E `union` L0)); inversion Red; subst.
-      specialize (H3 x ltac:(clear - H11; fsetdec)).
-      apply typing_state with (E := [(x, bind_typ (typ_capt (free_for_cv e1) (typ_arrow V0 T1)))] ++ E) (T := U0); simpl.
-      * SSCase "store_typing".
-        apply typing_store_cons.
-        -- assumption.
-        -- eapply typing_abs...
-        -- clear - H11; fsetdec.
-      * SSCase "eval_typing".
-        rewrite_env (empty ++ [(x, bind_typ (typ_capt (free_for_cv e1) (typ_arrow V0 T1)))] ++ E).
-        apply eval_typing_weakening...
-        applys typing_regular H3.
-      * SSCase "typing".
-        apply H3.
-  - Case "typing_app".
-    clear IHTyp1 IHTyp2.
-    destructs typing_var_inversion Typ1 as [[C [P [fBinds fPSubArr]]] | [X [fBiEnds XSubArr]]].
-    + assert (PSubT1T2 : sub_pre E P (typ_arrow T1 T2)) by (inversion fPSubArr; subst; eauto* ).
-      (* REVIEW: I don't think the following holds but:
-         We have `Γ ⊢ f : C (∀ (x : T1) → T2 x)`
-         If `f ∈ (fv_ct T1 ∪ fv_ct T2)`, we could possibly remove `f` from the
-         capture sets of `T1` and `T2` and lift the dependency on `f` by
-         `Γ ⊢ C <: C ∪ {f}` so that `Γ ⊢ f : (C ∪ {f}) (∀ (x : T1) → T2' x)`
-         where `T1'` and `T2'` are `T1` and `T2` where the dependency on `f`
-         has been removed.
-      *)
-      assert (NotIn : f `~in`A (fv_ct T1 `u`A fv_ct T2)).
-      { admit. }
-      destruct (binds_sub_arrow_implies_store_abs' _ _ _ _ _ _ _ StoreTyp fBinds NotIn PSubT1T2) as [S1 [e [abs_value [fStores T1SubS1]]]].
-      assert (AbsTyp : typing E (exp_abs S1 e) (typ_capt Cf (typ_arrow T1 T2))) by applys stores_preserves_typing StoreTyp fStores Typ1.
-      destruct (typing_inv_abs _ _ _ _ AbsTyp T1 T2 Cf) as [P1 [S2 [L' P2]]].
-      eapply sub_reflexivity with (Ap := dom E) (Am := dom E)...
-      1,2: clear; fsetdec.
-      specialize (Red (dom E `u`A L')); inversion Red; subst.
-      * SCase "red_lift".
-        inversion v_value.
-      * SCase "red_app".
-        eapply typing_state with (E := E) (T := open_ct T2 (`cset_fvar` x))...
-        destruct (P2 y)...
-           
-        apply typing_sub with (S := open_ct S2 (`cset_fvar` x)). 
-        Search (typing _ (open_ve _ _ _) (open_ct _ _)).
-    inversion EvalTyp; subst.
-    + SCase "typing_eval_nil".
-      specialize (Red {}A); inversion Red; subst.
-    + SCase "typing_eval_cons".
-      admit.
-
-
-    destruct (typing_of_var_comes_from_binds _ _ _ Typ1) as [TFun [fBinds SsubT]].
-    destruct (binds_sub_arrow_implies_store_abs _ _ _ _ _ _ _ StoreTyp fBinds SsubT) as [U' [e [abs_value [S_stores_abs T1_sub_U]]]].
-    assert (abs_typing : typing E (exp_abs U' e) (typ_capt Cf (typ_arrow T1 T2))).
-    { apply stores_preserves_typing with (S := S) (E := E) (x := f) (v_value := abs_value)... }
-    destruct (typing_inv_abs _ _ _ _ abs_typing T1 T2 Cf) as [P1 [S2 [L' P2]]].
-    eapply sub_reflexivity...
-    1,2: clear; fsetdec.
-    inversion EvalTyp; subst.
-    + SCase "final".
-      specialize (Red (dom E `u`A L' `u`A fv_ct S2 `u`A (`cset_fvars` (cv U')) `u`A fv_ve (open_ve e x (cv U')))); inversion Red; subst.
-      assert (arg_typing : typing E v T1).
-      { eapply stores_preserves_typing with (x := x) (v_value := v_value)... }
-      assert (exp_abs U' e = exp_abs U0 e0) by applys stores_unique S_stores_abs H7.
-      inversion H2; subst.
-      clear H2.
-      eapply typing_state with (E := E) (T := open_ct T2 (cv T1')); simpl.
-      * SSCase "store_typing".
-        assumption.
-      * SSCase "eval_typing".
-        apply typing_eval_nil...
-      * SSCase "typing".
-        destruct (P2 x) as [xU_E_e_S2 [WfS2 S2subV]]...
-        rewrite_env (empty ++ E).
-        apply typing_sub with (S := open_ct S2 (cv U0))...
-        -- apply typing_strengthening with (x := x) (U := U0).
-           ++ clear - H9; repeat apply notin_union...
-              apply notin_open_ct_rec_fv_ct with (c := cv U0).
-              fsetdec.
-           ++ admit.
-        -- admit.   
-    + SCase "cont".
-      specialize (Red (dom E `u`A L `u`A L' `u`A fv_ve (open_ve e x Cf))); inversion Red; subst.
-      * SSCase "red_lift".
-        inversion v_value.
-      * SSCase "red_app".
-        assert (arg_typing : typing E v T1).
-        { eapply stores_preserves_typing with (x := x) (v_value := v_value)... }
-        eapply typing_state with (E := E) (T := open_ct T2 (cv T1')); simpl...
-        assert (exp_abs U' e = exp_abs U1 e0) by applys stores_unique S_stores_abs H7.
-        inversion H2; subst.
-        clear H2.
-        destruct (P2 x ltac:(fsetdec)).
-        rewrite_env (empty ++ E).
-        apply typing_sub with (S := open_ct S2 (cv T1')).
-        -- apply typing_strengthening with (x := x) (U := U1).
-           ++ clear - H9; repeat apply notin_union...
-              all: admit.
-           ++ admit.
-        -- admit.
-  - Case "typing_let".
-    specialize (Red (dom E `union` L)); inversion Red; subst.
-    * SSCase "red_lift".
-      inversion v_value.
-    * SSCase "red_let_var".
-      eapply typing_state with (E := [(x, bind_typ T1)] ++ E) (T := T2); simpl.
-      -- apply typing_store_cons...
-      -- rewrite_env (empty ++ [(x, bind_typ T1)] ++ E).
-         assert (WfEnv : wf_env ([(x, bind_typ T1)] ++ E)) by applys typing_regular (H x ltac:(fsetdec)).
-         inversion WfEnv; subst.
-         apply eval_typing_weakening...
-      -- apply H...
-    * SSCase "red_let_exp".
-      eapply typing_state with (E := E) (T := T1); simpl.
-      -- assumption.
-      -- apply typing_eval_cons with (L := L) (U := T2)...
-      -- assumption.
-  - Case "typing_tabs".
-    inversion EvalTyp; subst.
-    + SCase "typing_eval_nil".
-      specialize (Red {}A); inversion Red.
-    + SCase "typing_eval_cons".
-      specialize (Red (dom E `union` L0)); inversion Red; subst.
-      specialize (H3 x ltac:(clear - H11; fsetdec)).
-      apply typing_state with (E := [(x, bind_typ (typ_capt (free_for_cv e1) (typ_all V0 T1)))] ++ E) (T := U0); simpl.
-      * SSCase "store_typing".
-        apply typing_store_cons.
-        -- assumption.
-        -- eapply typing_tabs...
-        -- clear - H11; fsetdec.
-      * SSCase "eval_typing".
-        rewrite_env (empty ++ [(x, bind_typ (typ_capt (free_for_cv e1) (typ_all V0 T1)))] ++ E).
-        apply eval_typing_weakening...
-        applys typing_regular H3.
-      * SSCase "typing".
-        apply H3.
-  - Case "typing_tapp".
-    admit.
-  - Case "typing_sub".
-    apply IHTyp...
-    apply eval_typing_contravariant.
-Admitted.   
-
-  inversion Step; subst; inversion TypState; subst.
-  all: try rename select (typing _ _ _ T) into Typ.
-  all: try rename select (typing _ _ _ T0) into Typ.
-  all: try rename select (typing_ctx _ _ _ T) into TypCtx.
-  all: try rename select (typing_ctx _ _ _ T0) into TypCtx.
-
-  Local Ltac solve_it_ctx := dependent induction TypCtx; hint; repeat (econstructor; hint).
-  Local Ltac solve_it_typ := dependent induction Typ; hint; repeat (econstructor; hint).
-
-  - Case "step-app".
-    solve_it_typ.
-  - Case "step-tapp".
-    solve_it_typ.
-    admit. (* T1 not universal, T <: T1 --> T not universal *)
-  - Case "step-fun->arg".
-    solve_it_ctx.
-  - Case "step-throw".
-    solve_it_typ.
-  - Case "step-handler->arg".
-    solve_it_ctx.
-  - Case "step-app".
-    assert (no_type_bindings empty) by (eauto using typing_ctx_free_tvar).
-    dependent induction TypCtx...
-
-    rename select (typing _ _ (exp_abs _ _) _) into TypAbs.
-    forwards (Sub & S2 & L & TypingX): typing_inv_abs TypAbs T1 T2 C...
-    1: { eauto using sub_reflexivity. }
-
-    pick fresh x.
-    destruct (TypingX x) as (TypingX' & Wf & SubS2).
-    1: { notin_solve. }
-
-    eapply typ_step...
-    rewrite (subst_ee_intro x) by notin_solve.
-    rewrite (subst_ct_intro x) by notin_solve.
-    assert (wf_typ_in empty T1') as WfTypV by eauto.
-    assert (wf_typ_in empty T1)  as WfTypT by eauto.
-    (**
-      E - environment
-      x - fresh atom
-      v - argument/value
-      e0 - body of abstraction (\lambda T e0)
-    *)
-    forwards (C' & P' & ?): inversion_toplevel_type WfTypV; subst...
-    forwards (C'' & P'' & ?): inversion_toplevel_type WfTypT; subst...
-
-    eapply typing_through_subst_ee' with (Ap := dom empty `union` singleton x) (Am := dom empty); trivial.
-    3,4: simpl_env; clear_frees; fsetdec.
-    (* 3: notin_solve. *)
-    + (* typing *)
-      rewrite_nil_concat.
-      eapply typing_narrowing_typ...
-      eapply typing_sub...
-      rewrite_nil_concat.
-      eapply typing_narrowing_typ...
-    + rewrite_nil_concat.
-      eapply wf_typ_narrowing_typ_base with (V := T); simpl_env...
-    + (* wf_cset free_for_cv *)
-      rename select (typing empty _ v _) into TypV.
-      forwards WfFvV: typing_cv TypV...
-    + inversion WfTypV. (* wf_cset C *)
-      rename select (wf_cset empty _ C') into WfC.
-      applys wf_cset_set_weakening WfC...
-  - Case "step-tapp".
-    dependent induction TypCtx...
-    econstructor...
-
-    rename select (typing _ _ (exp_tabs _ _) _) into TypTabs.
-    forwards (Sub & S2 & L & TypingX): typing_inv_tabs TypTabs T0 T3.
-    1: { eauto using sub_reflexivity. }
-
-    pick fresh x.
-    destruct (TypingX x) as [Typ' SubS2]...
-    rewrite (subst_te_intro x)...
-    rewrite (subst_tt_intro x)...
-    rewrite_env (map (subst_tb x T2) empty ++ empty).
-    apply (typing_through_subst_te T0)...
-  - assert (no_type_bindings empty) by (eauto using typing_ctx_free_tvar).
-    Notation "#H" := CCsub_Definitions.H.
-    dependent induction Typ...
-    unfold Signatures.singleton_list.
-    pick fresh x.
-    rename H2 into HH'.
-    forwards HH: HH' x. 1: { notin_solve. }
-    note (wf_env ((x, bind_typ (typ_capt {*} (typ_ret T))) :: empty)).
-    note (wf_typ_in empty (typ_capt {*} (typ_ret T))) as WfTypRet.
-    rename select (wf_pretyp empty _ _ (typ_ret T)) into WfT.
-    rewrite_env (empty ++ [(x, bind_typ (typ_capt {*} (typ_ret T)))] ++ empty) in HH.
-    replace Q with (nil ++ Q) in HH...
-    apply (typing_weakening_sig [(l, bind_sig (typ_capt {*} (typ_ret T)))]) in HH.
-    2: {
-      Signatures.simpl_env.
-      assert (wf_sig Q). {
-        pick fresh y for L.
-        eapply typing_regular_sig.
-        applys HH' y; trivial.
-      }
-      econstructor; simpl; trivial.
-      (* - (* here we need to know that T is wellformed in the empty environment. *) *)
-      (*   admit. *)
-      - forwards EQ: typing_ctx_calculates_bound_capabilities TypCtx.
-        rewrite EQ.
-        lsetdec.
-    }
-    rename HH into HH''.
-    forwards HH: typing_narrowing_typ (`cset_lvar` l) (typ_ret T) HH''. 1: {
-      constructor.
-      - apply subcapt_universal...
-      - eapply sub_pre_reflexivity...
-    }
-    apply typing_through_subst_ee with (u := (exp_lvar l)) in HH.
-    2: { eauto. }
-    2: {
-      simpl free_for_cv.
-      eapply typing_lvar...
-      Signatures.simpl_env.
-      assert (wf_sig Q). {
-        pick fresh y for L.
-        eapply typing_regular_sig.
-        applys HH' y; trivial.
-      }
-      econstructor; simpl; trivial.
-      (* - (* here we need to know that T is wellformed in the empty environment. *) *)
-      (*   admit. *)
-      - forwards EQ: typing_ctx_calculates_bound_capabilities TypCtx.
-        rewrite EQ.
-        lsetdec.
-    }
-    simpl in HH; simpl_env in HH; unfold Signatures.singleton_list in HH.
-    rewrite <- subst_ee_intro in HH by notin_solve.
-    rewrite <- subst_ct_fresh in HH. 2: {
-      (* inversion WfTypRet. *)
-      assert (x `~in`A dom empty). {
-        assert (wf_env ([(x, bind_typ (typ_capt {*} (typ_ret T)))] ++ empty)) as HA by eauto.
-        inversion HA; trivial.
-      }
-      enough (x `~in`A (fv_tt T `u`A fv_ct T)) by notin_solve.
-      applys notin_fv_wf_pretyp WfT; trivial.
-    }
-
-    eapply typ_step...
-    + eapply typing_ctx_reset...
-      * destruct (`cset_uvar` (cv T)) eqn:EQ...
-        enough (empty |-sc {*} <: cv T) by contradiction.
-        constructor.
-        2: exact EQ.
-        assert (wf_typ_in empty T) by eauto.
-        eapply cv_wf...
-      * forwards EQ: typing_ctx_calculates_bound_capabilities TypCtx.
-        rewrite EQ.
-        lsetdec.
-  - dependent induction TypCtx...
-    clear IHTypCtx.
-    econstructor...
-    applys typing_strengthening_sig_absent_label Typ.
-    applys label_absent_from_cv_is_absent_from_fv Typ; trivial.
-  - dependent induction TypCtx...
-    clear IHTypCtx.
-    dependent induction H0.
-    + inversion H; subst.
-      1: {
-        rename select (typing _ _ (exp_lvar l) _) into HH.
-        forwards (? & ? & ?): typing_inversion_lvar HH.
-        congruence.
-       }
-      inversion select (sub_pre _ _ (typ_ret Targ)); subst.
-      applys IHtyping l T1 C1...
-    + econstructor...
-  - solve_it_ctx.
-  - solve_it_ctx.
-  - solve_it_ctx.
-  - solve_it_ctx.
-  - solve_it_ctx.
-  - dependent induction TypCtx...
-    rename select (typing _ _ (exp_lvar l1) _) into TypLvar.
-    clear IHTypCtx.
-    dependent induction TypLvar.
-    1: {
-      inversion select (sub _ S _); subst.
-      1: {
-        rename select (typing _ _ (exp_lvar l1) _) into HH.
-        forwards (? & ? & ?): typing_inversion_lvar HH.
-        congruence.
-      }
-      inversion select (sub_pre _ _ (typ_ret R)); subst.
-      applys IHTypLvar T l2 T1...
-    }
-    assert (Signatures.binds l1 (bind_sig (typ_capt C0 (typ_ret R))) Q) as BndL1. {
-      rename select (Signatures.binds l1 _ _) into HA.
-      Signatures.binds_cases HA...
-    }
-    econstructor...
-    + rename select (typing _ _ v R) into TypV.
-      applys typing_strengthening_sig_absent_label TypV.
-      applys label_absent_from_cv_is_absent_from_fv TypV; trivial.
-      * applys extract_nontopness BndL1...
-      * assert (l2 `~in`L fv_lt (typ_capt C0 (typ_ret R))). {
-          applys notin_fv_ld_is_notin_fv_lt_of_bind_sig BndL1...
-        }
-        simpl in *.
-        destruct R; simpl in *; lsetdec.
-  - dependent induction TypCtx...
-    clear IHTypCtx.
-
-    rename select (typing _ _ (exp_lvar l) _) into TypLvar.
-    dependent induction TypLvar.
-    + inversion select (sub _ S _); subst.
-      1: {
-        rename select (typing _ _ (exp_lvar l) _) into HH.
-        forwards (? & ? & ?): typing_inversion_lvar HH.
-        congruence.
-      }
-      inversion select (sub_pre _ _ (typ_ret R)); subst.
-      applys IHTypLvar T l TypCtx T1...
-    + rename select (Signatures.binds _ _ _) into BndA.
-      assert (Signatures.binds l (bind_sig (typ_capt {*} (typ_ret T)))
-                               ([(l, bind_sig (typ_capt {*} (typ_ret T)))] ++ Q)) as BndA' by eauto.
-      forwards EQ: binds_sig_unique BndA BndA'.
-      inversion EQ; subst; clear EQ BndA'.
-      rename select (typing _ _ v T) into TypV.
-      forwards: typing_strengthening_sig_absent_label TypV.
-      1: {
-        applys label_absent_from_cv_is_absent_from_fv TypV...
-      }
-      econstructor...
+    destructs typing_inv_app NTB Typ as [C [T1 [T2 [fTyp [xTyp T2SubT]]]]].
+    destructs stores_preserves_typing StoreTyp H fTyp as [D [Q [absTyp [fBinds [e0SubD QSubP]]]]].
+    simpl in absTyp, e0SubD.
+    destruct (typing_inv_abs _ _ _ _ absTyp T1 T2 (free_for_cv e0)) as [T1SubU0 [S2 [L ?]]].
+    + apply sub_capt...
+      apply subcapt_reflexivity with (A := dom E)...
+      clear; fsetdec.
+    + pick fresh z and specialize H1.
+      destruct H1 as [e0Typ [WfT2 S2SubT2]].
+      eapply typing_state with (E := E) (T := open_ct T2 (`cset_fvar` x))...
+      * eapply eval_typing_sub...
+        apply sub_reflexivity with (Ap := dom E) (Am := dom E)...
+        applys eval_typing_regular EvalTyp.
+        all: clear; fsetdec.
+      * apply typing_sub with (S := open_ct S2 (`cset_fvar` x)).
+        -- apply typing_through_open_ve_typing with (y := z) (U := U0)...
+        -- rewrite_env (map (subst_cb z (`cset_fvar` x)) empty ++ E).
+           replace (open_ct S2 (`cset_fvar` x))
+              with (subst_ct z (`cset_fvar` x) (open_ct S2 (`cset_fvar` z)))
+              by (symmetry; apply subst_ct_intro; clear - Fr; fsetdec).
+           replace (open_ct T2 (`cset_fvar` x))
+              with (subst_ct z (`cset_fvar` x) (open_ct T2 (`cset_fvar` z)))
+              by (symmetry; apply subst_ct_intro; clear - Fr; fsetdec).
+           eapply sub_through_subst_ct...
+           clear - xTyp NTB.
+           destructs typing_var_inversion' NTB xTyp as [C [P [D [Q [Eq [PSubQ [xSubD Binds]]]]]]].
+           subst.
+           simpl...
+  - Case "red_tapp". 
+    destructs typing_tapp_inversion NTB Typ as [C [T1 [T2 [xTyp [T0SubT1 T2SubT]]]]].
+    destructs stores_preserves_typing StoreTyp H xTyp as [D [Q [tabsTyp [xBinds [e0SubD QSubP]]]]].
+    simpl in tabsTyp, e0SubD.
+    destruct (typing_inv_tabs _ _ _ _ tabsTyp T1 T2 (free_for_cv e0)) as [T1SubU0 [S2 [L ?]]].
+    + apply sub_capt...
+      apply subcapt_reflexivity with (A := dom E)...
+      clear; fsetdec.
+    + pick fresh z and specialize H1.
+      destruct H1 as [WfS2 S2SubT2].
+      eapply typing_state with (E := E) (T := open_tt T2 T0)...
+      * eapply eval_typing_sub...
+        apply sub_reflexivity with (Ap := dom E) (Am := dom E)...
+        applys eval_typing_regular EvalTyp.
+        all: clear; fsetdec.
+      * apply typing_through_open_te with (Y := z) (P := T0) (Q := T1)...
+        admit.
 Admitted.
 
-(* ********************************************************************** *)
-(** * #<a name="progress"></a># Progress *)
+Lemma binds_implies_store : forall S E x T,
+  store_typing S E ->
+  binds x (bind_typ T) E ->
+  exists v v_value, stores S x v v_value.
+Proof with eauto*.
+  intros * StoreTyp Binds.
+  induction StoreTyp.
+  - Case "typing_store_nil".
+    inversion Binds.
+  - Case "typing_store_cons".
+    binds_cases Binds.
+    + SCase "x in E".
+      destruct (IHStoreTyp H1) as [w [w_value Stores]].
+      exists w, w_value.
+      apply binds_tail...
+    + SCase "x = x0".
+      exists v, v_value.
+      apply binds_head...
+Qed. 
 
 (* ********************************************************************** *)
-(** ** Progress (16) *)
+(** ** Canonical forms (14) *)
 
-Lemma canonical_form_lvar : forall e Q C R,
-  value e ->
-  empty @ Q |-t e ~: (typ_capt C (typ_ret R)) ->
-  exists l, e = exp_lvar l.
-Proof with eauto.
-  intros * Val Typ.
-  dependent induction Typ; try solve [inversion Val]...
-  inversion select (sub _ S _); subst.
-  1: {
-    inversion select (binds _ _ empty).
-  }
-  inversion select (sub_pre _ _ (typ_ret R)); subst.
-  eapply IHTyp...
-Qed.
-
-Lemma progress_value_step : forall v k,
+Lemma canonical_form_abs' : forall E v C U1 U2,
+  no_type_bindings E ->
   value v ->
-  typing_state empty 〈 v | k 〉 ->
-  done 〈 v | k 〉 \/ exists s2, 〈 v | k 〉 --> s2.
-Proof with eauto.
-  intros * Val Typ.
-  inversion Typ; subst.
-  dependent induction H2.
-  - left; constructor...
-  - right...
-  - forwards (V & e1 & ?): canonical_form_abs H0...
-    subst.
-    right...
-  - forwards (V & e1 & ?): canonical_form_tabs H3...
-    subst.
-    right...
-  - right...
-  - forwards (? & ?): canonical_form_lvar H3...
-  - forwards (? & ?): canonical_form_lvar H0...
-    subst.
-    right...
-  - eauto.
-Qed.
+  typing E v (typ_capt C (typ_arrow U1 U2)) ->
+  exists S1 e, v = exp_abs S1 e
+             /\ sub E U1 S1
+             /\ exists L, forall x, x `~in`A L ->
+                  typing ([(x, bind_typ S1)] ++ E) (open_ve e x (`cset_fvar` x)) (open_ct U2 (`cset_fvar` x)).
+Proof with eauto*.
+  intros * NTB Val Typ.
+  remember (typ_arrow U1 U2).
+  revert U1 U2 Heqp.
+  assert (WfEnv : wf_env E) by applys typing_regular Typ.
+  dependent induction Typ; intros U1 U2 Eq; subst; try solve [ inversion Val | inversion Eq ].
+  - inversion Eq; subst.
+    exists U1, e1.
+    repeat split...
+    eapply sub_reflexivity...
+  - inversion H; subst.
+    + contradict H0; apply (NTB X U).
+    + inversion H5; subst.
+      destruct (IHTyp C1 NTB Val (typ_arrow S1 S2) eq_refl WfEnv S1 S2 eq_refl) as [S' [e' [Eq [Sub [L' ?]]]]].
+      exists S', e'.
+      repeat split...
+      * apply sub_transitivity with (Q := S1)...
+      * exists (L `u`A L').
+        intros x NotIn.
+        rewrite_env (empty ++ [(x, bind_typ S')] ++ E).
+        apply typing_sub with (S := open_ct S2 (`cset_fvar` x))...
+        admit.
+Admitted.
 
-Lemma progress_step : forall s1,
-  typing_state empty s1 ->
-  done s1 \/ exists s2, s1 --> s2.
-Proof with eauto.
-  intros * Typ.
-  inversion Typ; subst.
-  2: {
-    dependent induction H...
-    - dependent induction H1...
-      2: {
-        inversion H1.
-      }
-      inversion select (sub _ S _); subst.
-      1: {
-        rename select (typing _ _ (exp_lvar l) _) into HH.
-        forwards (? & ? & ?): typing_inversion_lvar HH.
-        congruence.
-      }
-      inversion select (sub_pre _ _ (typ_ret R)); subst.
-      applys IHtyping l C1 T1...
-    - right.
-      destruct (l0 ==== l); subst.
-      + eexists.
-        apply step_unwind_match_frame.
-      + eexists...
-  }
-  dependent induction H0.
-  - inversion select (binds _ _ _).
-  - inversion select (binds _ _ _).
-  - assert (value (exp_abs V e1)). {
-      assert (empty @ Q |-t (exp_abs V e1) ~: (typ_capt (free_for_cv e1) (typ_arrow V T1))). {
-        econstructor...
-      }
-      eauto.
+Lemma canonical_form_tabs' : forall E v C U1 U2,
+  no_type_bindings E ->
+  value v ->
+  typing E v (typ_capt C (typ_all U1 U2)) ->
+  exists S1 e, v = exp_tabs S1 e
+             /\ sub E U1 S1
+             /\ exists L, forall X, X `~in`A L ->
+                  typing ([(X, bind_sub S1)] ++ E) (open_te e X) (open_tt U2 X).
+Proof with eauto*.
+  intros * NTB Val Typ.
+  remember (typ_all U1 U2).
+  revert U1 U2 Heqp.
+  assert (WfEnv : wf_env E) by applys typing_regular Typ.
+  dependent induction Typ; intros U1 U2 Eq; subst; try solve [ inversion Val | inversion Eq ].
+  - inversion Eq; subst.
+    exists U1, e1.
+    repeat split...
+    eapply sub_reflexivity...
+  - inversion H; subst.
+    + contradict H0; apply (NTB X U).
+    + inversion H5; subst.
+      destruct (IHTyp C1 NTB Val (typ_all S1 S2) eq_refl WfEnv S1 S2 eq_refl) as [S' [e' [Eq [Sub [L' ?]]]]].
+      exists S', e'.
+      repeat split...
+      * apply sub_transitivity with (Q := S1)...
+      * exists (L `u`A L').
+        intros X NotIn.
+        apply typing_sub with (S := open_tt S2 X)...
+        specialize (H11 X ltac:(clear - NotIn; fsetdec)).
+        rewrite_env (empty ++ [(X, bind_sub S')] ++ E).
+        eapply sub_narrowing with (Q := U1)...
+        admit.
+Admitted.
+
+Lemma progress : forall s V, 
+  state_typing s V ->
+  state_final s \/ exists s', red s s'.
+Proof with eauto*.
+  intros * [S K e E T U StoreTyp EvalTyp Typ].
+  assert (NTB : no_type_bindings E) by applys store_typing_no_type_bindings StoreTyp.
+  induction Typ.
+  - Case "typing_var_tvar".
+    assert (WfX : wf_typ_in E X) by (apply wf_env_bound_implies_wf_typ with (x := x); eauto).
+    inversion WfX; subst.
+    contradict H2.
+    apply NTB.
+  - Case "typing_var".
+    inversion EvalTyp; subst.
+    + left; apply final_state, answer_var.
+    + right.
+      exists ⟨ S | K0 | open_ve k x (`cset_fvar` x) ⟩.
+      destructs binds_implies_store StoreTyp H0 as [v [v_value Stores]].
+      eapply red_let_var...
+  - Case "typing_abs".
+    assert (Val : value (exp_abs V0 e1)).
+    { apply value_abs.
+      apply expr_abs with (L := L).
+      * eapply type_from_wf_typ, H.
+      * intros x NotIn.
+        specialize (H1 x NotIn).
+        applys typing_regular H1.
     }
-    eapply progress_value_step...
-  - right...
-  - assert (value (exp_tabs V e1)). {
-      assert (empty @ Q |-t (exp_tabs V e1) ~: (typ_capt (free_for_cv e1) (typ_all V T1))). {
-        econstructor...
-      }
-      eauto.
+    inversion EvalTyp; subst.
+    + left; apply final_state, answer_val, Val.
+    + right.
+      pick fresh z for (dom S).
+      exists ⟨ [(z, store (exp_abs V0 e1) Val)] ++ S | K0 | open_ve k z (`cset_fvar` z) ⟩.
+      apply red_lift, Fr.
+  - Case "typing_app".
+    right.
+    destructs typing_var_inversion' NTB Typ1 as [C [P [D [Q [Eq [PSubQ [fSubD Binds]]]]]]].
+    inversion Eq; subst; clear Eq.
+    destructs binds_implies_store StoreTyp Binds as [abs [absValue Stores]].
+    destructs stores_preserves_typing StoreTyp Stores Typ1 as [Cf [Qf [absTyp [fBinds [absSubCf QfSubT1T2]]]]].
+    eapply typing_sub in absTyp.
+    2: apply sub_capt...
+    destructs canonical_form_abs' NTB absValue absTyp as [U0 [e [Eq [T1SubU [L ?]]]]]; subst.
+    exists ⟨ S | K | open_ve e x (`cset_fvar` x) ⟩.
+    destructs typing_var_inversion' NTB Typ2 as [C' [P' [D' [Q' [Eq [P'SubQ' [xSubD' Binds']]]]]]].
+    destructs binds_implies_store StoreTyp Binds' as [v [v_value Stores']].
+    eapply red_app...
+  - Case "typing_let".
+    right.
+    pick fresh z for (dom S).
+    assert (k_scope : scope k).
+    { econstructor.
+      intros x NotIn.
+      specialize (H x NotIn).
+      applys typing_regular H.
     }
-    eapply progress_value_step...
-  - right...
-  - apply IHtyping...
-    applys typing_ctx_sub H1...
-  - pick fresh label l for (Signatures.dom (bound_capabilities k)
-                                           `u`L fv_ld (bound_capabilities k)
-                                           `u`L `cset_lvars` (cv T1)).
-    right; eexists.
-    eapply step_try with (l := l).
-    all: lsetdec.
-  - right...
-  - assert (value (exp_lvar l)) by eauto.
-    eapply progress_value_step...
-Qed.
+    exists ⟨ S | cont k k_scope :: K | e ⟩.
+    apply red_let_exp.
+  - Case "typing_tabs".
+    assert (Val : value (exp_tabs V0 e1)).
+    { apply value_tabs.
+      apply expr_tabs with (L := L).
+      * eapply type_from_wf_typ, H.
+      * intros x NotIn.
+        specialize (H1 x NotIn).
+        applys typing_regular H1.
+    }
+    inversion EvalTyp; subst.
+    + left; apply final_state, answer_val, Val.
+    + right.
+      pick fresh z for (dom S).
+      exists ⟨ [(z, store (exp_tabs V0 e1) Val)] ++ S | K0 | open_ve k z (`cset_fvar` z) ⟩.
+      apply red_lift, Fr.
+  - Case "typing_tabs".
+    right.
+    destructs typing_var_inversion' NTB Typ as [C' [P' [D' [Q' [Eq [P'SubQ' [xSubD' Binds]]]]]]].
+    inversion Eq; subst; clear Eq.
+    destructs binds_implies_store StoreTyp Binds as [abs [tabsValue Stores]].
+    destructs stores_preserves_typing StoreTyp Stores Typ as [Cf [Qf [tabsTyp [xBinds [tabsSubCf QfSubT1T2]]]]].
+    eapply typing_sub in tabsTyp.
+    2: apply sub_capt...
+    destructs canonical_form_tabs' NTB tabsValue tabsTyp as [U0 [e [Eq [T1SubU [L ?]]]]]; subst.
+    exists ⟨ S | K | open_te e T ⟩.
+    eapply red_tapp...
+  - Case "typing_sub".
+    apply IHTyp...
+    eapply eval_typing_sub with (S1 := T) (T1 := U)...
+    eapply sub_reflexivity...
+    applys eval_typing_regular EvalTyp.
+    all: clear; fsetdec.
+  Qed.
